
@prefix rdf: <http://www.w3.org/1999/02/22-rdf-syntax-ns#> .
@prefix rdfs: <http://www.w3.org/2000/01/rdf-schema#> .
@prefix owl: <http://www.w3.org/2002/07/owl#> .
@prefix sh: <https://www.w3.org/ns/shacl#> .
@prefix W3C: <https://www.w3.org/standards/semanticweb#> .
@prefix xs: <http://www.w3.org/2001/XMLSchema#> .
@prefix xsd: <http://www.w3.org/2001/XMLSchema#> .
@prefix dcterms: <http://purl.org/dc/terms/> .
@prefix dc: <http://purl.org/dc/elements/1.1/> .
@prefix schema: <https://schema.org#> .
@prefix iana: <https://www.iana.org/assignments/media-types#> .
@prefix foaf: <http://xmlns.com/foaf/spec/#> .
@prefix FMC: <http://fmc-modeling.org#> .
@prefix IR: <https://www.adesso.de/de/impulse/interaction-room/index.jsp#> .
@prefix IREB: <https://www.ireb.org/en/downloads#cpre-glossary> .
@prefix ReqIF: <https://www.prostep.org/fileadmin/downloads/PSI_ImplementationGuide_ReqIF_V1-7.pdf#> .
@prefix ReqIF-WF: <https://www.prostep.org/fileadmin/downloads/Recommendation_ReqIF_V2_RZ3.pdf#> .
@prefix HIS: <https://www.itwissen.info/Herstellerinitiative-Software-Automotive-HIS.html#> .
@prefix oslc: <http://open-services.net/ns/core#> .
@prefix oslc_rm: <http://open-services.net/ns/rm#> .
@prefix oslc_cm: <http://open-services.net/ns/cm#> .
@prefix ArchiMate: <https://pubs.opengroup.org#> .
@prefix bpmn: <https://www.bpmn.org#> .
@prefix uml: <https://www.omg.org/spec/UML#> .
@prefix sysml: <https://www.omg.org/spec/SysML#> .
@prefix pig: <https://product-information-graph.org/metamodel#> .
@prefix DDP: <http://www.prostep.org/dictionary/2.0#> .
@prefix SpecIF: <https://specif.de/v1.1/schema#> .
@prefix sh: <http://www.w3.org/ns/shacl#> .

@prefix o: <https://product-information-graph.org/examples/ontology#> .
@prefix d: <https://product-information-graph.org/examples/SpecIF%20Classes%20with%20tiny%20example%20CRM.specif.specif#> .

#################################################################
# Project Metadata
#################################################################

d:
	rdf:type owl:Ontology ;
	rdfs:label "SpecIF Classes with tiny example CRM" ;
	rdfs:comment "A set of SpecIF Classes derived from a SpecIF Ontology for the domains SpecIF:DomainRequirementsEngineering, SpecIF:DomainSystemsEngineering, SpecIF:DomainSystemModelIntegration, SpecIF:DomainEnterpriseArchitecture with tiny example CRM."@en ;
	owl:imports <http://www.w3.org/1999/02/22-rdf-syntax-ns#> ,
		<http://www.w3.org/2000/01/rdf-schema#> ;
	dcterms:license <https://creativecommons.org/licenses/by-sa/4.0/> ;
	dcterms:createdAt "2025-09-24T13:59:01.617Z" .

#################################################################
### META-ONTOLOGY = PIG Metamodel (pig:)
#################################################################

pig:Organizer
	rdf:type owl:Class ;
	rdfs:label "Organizer" ;
	rdfs:comment "A PIG meta-model element used for organizing model-elements." .

pig:Entity
	rdf:type owl:Class ;
	rdfs:label "Entity" ;
	rdfs:comment "A PIG meta-model element used for entities (aka resources or artifacts)." .

pig:Relationship
	rdf:type owl:Class ;
	rdfs:label "Relationship" ;
	rdfs:comment "A PIG meta-model element used for reified relationships (aka predicates)." .

pig:eligibleSource
	rdf:type owl:ObjectProperty ;
	rdfs:domain pig:Relationship ;
	rdfs:range pig:Entity ;
	rdfs:label "has source" ;
	rdfs:comment "Connects the source of a reified relationship." .

pig:eligibleTarget
	rdf:type owl:ObjectProperty ;
	rdfs:domain pig:Relationship ;
	rdfs:range pig:Entity ;
	rdfs:label "has target" ;
	rdfs:comment "Connects the target of a reified relationship." .

pig:eligibleElement
	rdf:type owl:ObjectProperty ;
	rdfs:domain pig:Organizer ;
	rdfs:range [ owl:unionOf( pig:Entity pig:Relationship pig:Organizer )] ;
	rdfs:label "has element" ;
	rdfs:comment "References an entity, a relationship or a subordinated organizer." .

pig:lists
	rdfs:subPropertyOf pig:eligibleElement ;
	rdfs:domain pig:Outline ;
	rdfs:label "lists" ;
	rdfs:comment "Lists (references) an entity, a relationship or a subordinated organizer." .

pig:shows
	rdfs:subPropertyOf pig:eligibleElement ;
	rdfs:domain pig:View ;
	rdfs:range [ owl:unionOf( pig:Entity pig:Relationship )] ;
	rdfs:label "shows" ;
	rdfs:comment "Shows (references) an entity or a relationship." .

pig:depicts
	rdfs:subPropertyOf pig:eligibleElement ;
	rdfs:domain pig:View ;
	rdfs:range pig:Entity ;
	rdfs:label "depicts" ;
	rdfs:comment "Depicts an entity; inverse of uml:ownedDiagram." .

#################################################################
# Data Types with Enumerated Values
#################################################################

SpecIF:EngineeringDiscipline-Value
	rdf:type owl:Class ;
	rdfs:label "Engineering Discipline"@en ;
	rdfs:label "Ingenieurdisziplin"@de ;
	rdfs:label "Discipline d'ingénierie"@fr ;
	rdfs:comment "Enumerated Values for Ingenieurdisziplin" ;
	dcterms:modified "2023-03-06T08:27:59.451Z" ;
	owl:oneOf ( SpecIF:EngineeringDisciplineMechanics SpecIF:EngineeringDisciplineElectronics SpecIF:EngineeringDisciplineSoftware SpecIF:EngineeringDisciplineSafety SpecIF:EngineeringDisciplineSystem ) .
SpecIF:EngineeringDisciplineMechanics
	rdf:type SpecIF:EngineeringDiscipline-Value ;
	rdfs:label "Mechanics"@en ;
	rdfs:label "Mechanik"@de ;
	rdfs:label "Mecanique"@fr .
SpecIF:EngineeringDisciplineElectronics
	rdf:type SpecIF:EngineeringDiscipline-Value ;
	rdfs:label "Electronics"@en ;
	rdfs:label "Elektronik"@de ;
	rdfs:label "Électronique"@fr .
SpecIF:EngineeringDisciplineSoftware
	rdf:type SpecIF:EngineeringDiscipline-Value ;
	rdfs:label "Software"@en ;
	rdfs:label "Logiciel"@fr .
SpecIF:EngineeringDisciplineSafety
	rdf:type SpecIF:EngineeringDiscipline-Value ;
	rdfs:label "Safety"@en ;
	rdfs:label "Sicherheit"@de ;
	rdfs:label "Sécurité"@fr .
SpecIF:EngineeringDisciplineSystem
	rdf:type SpecIF:EngineeringDiscipline-Value ;
	rdfs:label "System Engineering"@en .

SpecIF:StakeholderGroup-Value
	rdf:type owl:Class ;
	rdfs:label "Stakeholder Group"@en ;
	rdfs:comment "Enumerated Values for Stakeholder Group" ;
	dcterms:modified "2023-03-10T07:48:02.442Z" ;
	owl:oneOf ( SpecIF:StakeholderGroupRegulation SpecIF:StakeholderGroupBusiness SpecIF:StakeholderGroupUser SpecIF:StakeholderGroupSystem SpecIF:StakeholderGroupOperation ) .
SpecIF:StakeholderGroupRegulation
	rdf:type SpecIF:StakeholderGroup-Value ;
	rdfs:label "Regulation"@en ;
	rdfs:comment "The stakeholder group 'Regulation' addressed by a requirement." .
SpecIF:StakeholderGroupBusiness
	rdf:type SpecIF:StakeholderGroup-Value ;
	rdfs:label "Business"@en ;
	rdfs:comment "The stakeholder group 'Business' addressed by a requirement." .
SpecIF:StakeholderGroupUser
	rdf:type SpecIF:StakeholderGroup-Value ;
	rdfs:label "User"@en ;
	rdfs:comment "The stakeholder group 'User' addressed by a requirement." .
SpecIF:StakeholderGroupSystem
	rdf:type SpecIF:StakeholderGroup-Value ;
	rdfs:label "System"@en ;
	rdfs:comment "The stakeholder group 'System' addressed by a requirement." .
SpecIF:StakeholderGroupOperation
	rdf:type SpecIF:StakeholderGroup-Value ;
	rdfs:label "Operation"@en ;
	rdfs:comment "The stakeholder group 'Operation' addressed by a requirement." .

SpecIF:Instantiation-Value
	rdf:type owl:Class ;
	rdfs:label "Instantiation" ;
	rdfs:comment "Enumerated Values for Instantiation" ;
	dcterms:modified "2025-06-28T12:46:58.743Z" ;
	owl:oneOf ( SpecIF:InstantiationAuto SpecIF:InstantiationUser SpecIF:InstantiationNever ) .
SpecIF:InstantiationAuto
	rdf:type SpecIF:Instantiation-Value ;
	rdfs:label "auto" ;
	rdfs:comment "The element class is instantiated automatically.This term defines a value of native property of a term. When a SpecIF class with the native property is generated, the default language of of the first value in 'Local Term' will be used. All others are ignored." .
SpecIF:InstantiationUser
	rdf:type SpecIF:Instantiation-Value ;
	rdfs:label "user" ;
	rdfs:comment "The element class can be instantiated by a user.This term defines a value of native property of a term. When a SpecIF class with the native property is generated, the default language of of the first value in 'Local Term' will be used. All others are ignored." .
SpecIF:InstantiationNever
	rdf:type SpecIF:Instantiation-Value ;
	rdfs:label "never" ;
	rdfs:comment "The element class is never instantiated. It is however extended by classes of the same category.This term defines a value of native property of a term. When a SpecIF class with the native property is generated, the default language of of the first value in 'Local Term' will be used. All others are ignored." .

SpecIF:LifecycleStatus-Value
	rdf:type owl:Class ;
	rdfs:label "Lifecycle"@en ;
	rdfs:label "Lebenszyklus"@de ;
	rdfs:label "Cycle de vie"@fr ;
	rdfs:comment "Enumerated Values for Lebenszyklus" ;
	dcterms:modified "2025-09-05T12:53:10.216Z" ;
	owl:oneOf ( SpecIF:LifecycleStatusInitial SpecIF:LifecycleStatusDrafted SpecIF:LifecycleStatusSubmitted SpecIF:LifecycleStatusApproved SpecIF:LifecycleStatusReady SpecIF:LifecycleStatusDone SpecIF:LifecycleStatusValidated SpecIF:LifecycleStatusReleased SpecIF:LifecycleStatusDeprecated SpecIF:LifecycleStatusWithdrawn SpecIF:LifecycleStatusPostponed SpecIF:LifecycleStatusRejected ) .
SpecIF:LifecycleStatusInitial
	rdf:type SpecIF:LifecycleStatus-Value ;
	rdfs:label "initial"@en .
SpecIF:LifecycleStatusDrafted
	rdf:type SpecIF:LifecycleStatus-Value ;
	rdfs:label "drafted"@en ;
	rdfs:label "entworfen"@de ;
	rdfs:label "rédigé"@fr .
SpecIF:LifecycleStatusSubmitted
	rdf:type SpecIF:LifecycleStatus-Value ;
	rdfs:label "submitted"@en ;
	rdfs:label "vorgelegt"@de ;
	rdfs:label "soumis"@fr .
SpecIF:LifecycleStatusApproved
	rdf:type SpecIF:LifecycleStatus-Value ;
	rdfs:label "approved"@en ;
	rdfs:label "genehmigt"@de ;
	rdfs:label "approuvé"@fr .
SpecIF:LifecycleStatusReady
	rdf:type SpecIF:LifecycleStatus-Value ;
	rdfs:label "ready"@en ;
	rdfs:label "bereit ('ready')"@de ;
	rdfs:comment "Meets the requirements of the 'Definition of Ready' of the agile development method." .
SpecIF:LifecycleStatusDone
	rdf:type SpecIF:LifecycleStatus-Value ;
	rdfs:label "done"@en ;
	rdfs:label "erledigt ('done')"@de ;
	rdfs:comment "Meets the requirements of the 'Definition of Done' of the agile development method." .
SpecIF:LifecycleStatusValidated
	rdf:type SpecIF:LifecycleStatus-Value ;
	rdfs:label "validated"@en ;
	rdfs:label "validiert"@de ;
	rdfs:label "validé"@fr .
SpecIF:LifecycleStatusReleased
	rdf:type SpecIF:LifecycleStatus-Value ;
	rdfs:label "released"@en ;
	rdfs:label "freigegeben"@de ;
	rdfs:label "publié"@fr .
SpecIF:LifecycleStatusDeprecated
	rdf:type SpecIF:LifecycleStatus-Value ;
	rdfs:label "deprecated"@en ;
	rdfs:label "veraltet"@de ;
	rdfs:label "dépassé"@fr .
SpecIF:LifecycleStatusWithdrawn
	rdf:type SpecIF:LifecycleStatus-Value ;
	rdfs:label "withdrawn"@en ;
	rdfs:label "zurückgezogen"@de ;
	rdfs:label "retiré"@fr .
SpecIF:LifecycleStatusPostponed
	rdf:type SpecIF:LifecycleStatus-Value ;
	rdfs:label "postponed"@en ;
	rdfs:label "aufgeschoben"@de ;
	rdfs:label "repoussé"@fr .
SpecIF:LifecycleStatusRejected
	rdf:type SpecIF:LifecycleStatus-Value ;
	rdfs:label "rejected"@en ;
	rdfs:label "abgelehnt"@de ;
	rdfs:label "rejeté"@fr .

SpecIF:Priority-Value
	rdf:type owl:Class ;
	rdfs:label "Priority"@en ;
	rdfs:label "Priorität"@de ;
	rdfs:label "Priorité"@fr ;
	rdfs:comment "Enumerated Values for Priorität" ;
	dcterms:modified "2025-09-05T12:40:27.574Z" ;
	owl:oneOf ( SpecIF:priorityHigh SpecIF:priorityRatherHigh SpecIF:priorityMedium SpecIF:priorityRatherLow SpecIF:priorityLow ) .
SpecIF:priorityHigh
	rdf:type SpecIF:Priority-Value ;
	rdfs:label "high"@en ;
	rdfs:label "hoch"@de ;
	rdfs:label "haut"@fr ;
	rdfs:comment "A value for property [[SpecIF:Priority]]." .
SpecIF:priorityRatherHigh
	rdf:type SpecIF:Priority-Value ;
	rdfs:label "rather high"@en ;
	rdfs:label "eher hoch"@de ;
	rdfs:label "plutôt haut"@fr ;
	rdfs:comment "A value for property [[SpecIF:Priority]]." .
SpecIF:priorityMedium
	rdf:type SpecIF:Priority-Value ;
	rdfs:label "medium"@en ;
	rdfs:label "mittel"@de ;
	rdfs:label "moyen"@fr ;
	rdfs:comment "A value for property [[SpecIF:Priority]]." .
SpecIF:priorityRatherLow
	rdf:type SpecIF:Priority-Value ;
	rdfs:label "rather low"@en ;
	rdfs:label "eher niedrig"@de ;
	rdfs:label "plutôt bas"@fr ;
	rdfs:comment "A value for property [[SpecIF:Priority]]." .
SpecIF:priorityLow
	rdf:type SpecIF:Priority-Value ;
	rdfs:label "low"@en ;
	rdfs:label "niedrig"@de ;
	rdfs:label "bas"@fr ;
	rdfs:comment "A value for property [[SpecIF:Priority]]." .

IREB:RequirementType-Value
	rdf:type owl:Class ;
	rdfs:label "Type"@en ;
	rdfs:label "Art"@de ;
	rdfs:comment "Enumerated Values for Art" ;
	dcterms:modified "2023-08-08T20:52:31.633Z" ;
	owl:oneOf ( o:V_RequirementType_0 o:V_RequirementType_1 IREB:FunctionalRequirement IREB:QualityRequirement IREB:Constraint o:V_RequirementType_5 ) .
o:V_RequirementType_0
	rdf:type IREB:RequirementType-Value ;
	rdfs:label "SpecIF:Feature" .
o:V_RequirementType_1
	rdf:type IREB:RequirementType-Value ;
	rdfs:label "SpecIF:UserStory" .
IREB:FunctionalRequirement
	rdf:type IREB:RequirementType-Value ;
	rdfs:label "Functional Requirement"@en ;
	rdfs:label "Funktionsanforderung"@de ;
	rdfs:label "Exigence de function"@fr ;
	rdfs:comment "A [[IREB:Requirement]] concerning a result of behavior that shall be provided by a function of a system (or of a component or service)."@en .
IREB:QualityRequirement
	rdf:type IREB:RequirementType-Value ;
	rdfs:label "Quality Requirement"@en ;
	rdfs:label "Qualitätsanforderung"@de ;
	rdfs:label "Exigence de qualité"@fr ;
	rdfs:comment "A [[IREB:Requirement]] that pertains to a quality concern that is not covered by functional requirements."@en .
IREB:Constraint
	rdf:type IREB:RequirementType-Value ;
	rdfs:label "Constraint"@en ;
	rdfs:label "Randbedingung"@de ;
	rdfs:label "Contrainte"@fr ;
	rdfs:comment "A [[IREB:Requirement]] that limits the solution space beyond what is necessary for meeting the given functional requirements and quality requirements."@en .
o:V_RequirementType_5
	rdf:type IREB:RequirementType-Value ;
	rdfs:label "SpecIF:PainPoint" .

ReqIF-WF:SupplierStatus-Value
	rdf:type owl:Class ;
	rdfs:label "Supplier Status"@en ;
	rdfs:label "Zustand Lieferant"@de ;
	rdfs:label "Statut coté Fournisseur"@fr ;
	rdfs:comment "Enumerated Values for Zustand Lieferant" ;
	dcterms:modified "2023-07-16T11:06:47.817Z" ;
	owl:oneOf ( ReqIF-WF:SupplierStatus.ToBeClarified ReqIF-WF:SupplierStatus.AgreedWithComment ReqIF-WF:SupplierStatus.Agreed ReqIF-WF:SupplierStatus.NotAgreed ReqIF-WF:SupplierStatus.DiscardedDeployed ) .
ReqIF-WF:SupplierStatus.ToBeClarified
	rdf:type ReqIF-WF:SupplierStatus-Value ;
	rdfs:label "to be clarified"@en ;
	rdfs:label "zu klären"@de ;
	rdfs:label "à préciser"@fr .
ReqIF-WF:SupplierStatus.AgreedWithComment
	rdf:type ReqIF-WF:SupplierStatus-Value ;
	rdfs:label "agreed with comment"@en ;
	rdfs:label "zugestimmt mit Kommentar"@de ;
	rdfs:label "approuvé avec commentaire"@fr .
ReqIF-WF:SupplierStatus.Agreed
	rdf:type ReqIF-WF:SupplierStatus-Value ;
	rdfs:label "agreed"@en ;
	rdfs:label "zugestimmt"@de ;
	rdfs:label "approuvé"@fr .
ReqIF-WF:SupplierStatus.NotAgreed
	rdf:type ReqIF-WF:SupplierStatus-Value ;
	rdfs:label "not agreed"@en ;
	rdfs:label "nicht zugestimmt"@de ;
	rdfs:label "non approuvé"@fr .
ReqIF-WF:SupplierStatus.DiscardedDeployed
	rdf:type ReqIF-WF:SupplierStatus-Value ;
	rdfs:label "discarded"@en ;
	rdfs:label "gelöscht"@de ;
	rdfs:label "écarté"@fr .

ReqIF-WF:CustomerStatus-Value
	rdf:type owl:Class ;
	rdfs:label "Customer Status"@en ;
	rdfs:label "Zustand Kunde"@de ;
	rdfs:label "Statut coté Client"@fr ;
	rdfs:comment "Enumerated Values for Zustand Kunde" ;
	dcterms:modified "2023-07-16T11:06:10.422Z" ;
	owl:oneOf ( ReqIF-WF:CustomerStatus.ToEvaluate ReqIF-WF:CustomerStatus.ToBeClarified ReqIF-WF:CustomerStatus.NotAccepted ReqIF-WF:CustomerStatus.Accepted ReqIF-WF:CustomerStatus.NotToEvaluate ReqIF-WF:CustomerStatus.ProposedToDiscard ReqIF-WF:CustomerStatus.Discarded ) .
ReqIF-WF:CustomerStatus.ToEvaluate
	rdf:type ReqIF-WF:CustomerStatus-Value ;
	rdfs:label "to evaluate"@en ;
	rdfs:label "zu evaluieren"@de ;
	rdfs:label "pour évaluer"@fr .
ReqIF-WF:CustomerStatus.ToBeClarified
	rdf:type ReqIF-WF:CustomerStatus-Value ;
	rdfs:label "to be clarified"@en ;
	rdfs:label "zu klären"@de ;
	rdfs:label "à préciser"@fr .
ReqIF-WF:CustomerStatus.NotAccepted
	rdf:type ReqIF-WF:CustomerStatus-Value ;
	rdfs:label "not accepted"@en ;
	rdfs:label "nicht akzeptiert"@de ;
	rdfs:label "non accepté"@fr .
ReqIF-WF:CustomerStatus.Accepted
	rdf:type ReqIF-WF:CustomerStatus-Value ;
	rdfs:label "accepted"@en ;
	rdfs:label "akzeptiert"@de ;
	rdfs:label "accepté"@fr .
ReqIF-WF:CustomerStatus.NotToEvaluate
	rdf:type ReqIF-WF:CustomerStatus-Value ;
	rdfs:label "not to evaluate"@en ;
	rdfs:label "nicht zu evaluieren"@de ;
	rdfs:label "ne pas évaluer"@fr .
ReqIF-WF:CustomerStatus.ProposedToDiscard
	rdf:type ReqIF-WF:CustomerStatus-Value ;
	rdfs:label "proposed to discard"@en ;
	rdfs:label "vorgesehen zu löschen"@de ;
	rdfs:label "proposé d'écarter"@fr .
ReqIF-WF:CustomerStatus.Discarded
	rdf:type ReqIF-WF:CustomerStatus-Value ;
	rdfs:label "discarded"@en ;
	rdfs:label "gelöscht"@de ;
	rdfs:label "écarté"@fr .

#################################################################
# Ontology - Property Classes
#################################################################

SpecIF:Diagram
	rdf:type owl:DatatypeProperty ;
	rdfs:label "Diagram"@en ;
	rdfs:label "Diagramm"@de ;
	rdfs:label "Diagramme"@fr ;
	rdfs:comment "A diagram illustrating the resource or a link to a diagram."@en .

SpecIF:Diagram-Shape
	rdf:type sh:PropertyShape ;
	sh:path SpecIF:Diagram ;
	sh:datatype xsd:string .

SpecIF:Notation
	rdf:type owl:DatatypeProperty ;
	rdfs:label "Notation"@en ;
	rdfs:comment "The notation used by a model diagram, e.g. 'BPMN 2.0', 'SysML Activity Diagram' or 'FMC Block Diagram'."@en .

SpecIF:Notation-Shape
	rdf:type sh:PropertyShape ;
	sh:path SpecIF:Notation ;
	sh:maxCount "1" ;
	sh:datatype xsd:string ;
	sh:maxLength "32" .

SpecIF:Vote
	rdf:type owl:DatatypeProperty ;
	rdfs:label "Vote" ;
	rdfs:comment "<p>A 'Vote' is an opinion referring to any resource or statement.</p>"@en .

SpecIF:Vote-Shape
	rdf:type sh:PropertyShape ;
	sh:path SpecIF:Vote ;
	sh:maxCount "1" ;
	sh:datatype xsd:integer ;
	sh:minInclusive "-1" ;
	sh:maxInclusive "1" .

dcterms:subject
	rdf:type owl:DatatypeProperty ;
	rdfs:label "Subject"@en ;
	rdfs:label "Thema"@de ;
	rdfs:label "Sujet"@fr ;
	rdfs:comment "<p>The topic of the resource. <small>(<i>source: <a href=\"http://purl.org/dc/elements/1.1/subject\">DCMI</a></i>)</small></p><p>Tag or keyword for a resource. Each occurrence of a dcterms:subject property denotes an additional tag for the resource. <small>(<i>source: <a href=\"http://open-services.net/\">OSLC</a></i>)</small></p>"@en .

dcterms:subject-Shape
	rdf:type sh:PropertyShape ;
	sh:path dcterms:subject ;
	sh:maxCount "1" ;
	sh:datatype xsd:string .

SpecIF:ownedBy
	rdf:type owl:DatatypeProperty ;
	rdfs:label "owned by" .

SpecIF:ownedBy-Shape
	rdf:type sh:PropertyShape ;
	sh:path SpecIF:ownedBy ;
	sh:maxCount "1" ;
	sh:datatype xsd:string ;
	sh:maxLength "32" .

SpecIF:Motivation
	rdf:type owl:DatatypeProperty ;
	rdfs:label "Motivation" .

SpecIF:Motivation-Shape
	rdf:type sh:PropertyShape ;
	sh:path SpecIF:Motivation ;
	sh:maxCount "1" ;
	sh:datatype xsd:string .

uml:Stereotype
	rdf:type owl:DatatypeProperty ;
	rdfs:label "Stereotype" ;
	rdfs:comment "<p>Describes the role or sub-type of a model-element. For example, a [[FMC:Actor]] may represent a <i>System Function</i>, a <i>System Component</i> or a <i>User Role</i>. Similarly, in the context of process modelling, a FMC:Actor may represent a <i>Process Step</i> or again a <i>User Role</i>. So, all of these are meaningful values for a FMC:Actor's property named uml:Stereotype.</p>" .

uml:Stereotype-Shape
	rdf:type sh:PropertyShape ;
	sh:path uml:Stereotype ;
	sh:maxCount "1" ;
	sh:datatype xsd:string .

uml:is_Service
	rdf:type owl:DatatypeProperty ;
	rdfs:label "is server"@en .

uml:is_Service-Shape
	rdf:type sh:PropertyShape ;
	sh:path uml:is_Service ;
	sh:maxCount "1" ;
	sh:datatype xsd:boolean .

uml:Flow_Direction
	rdf:type owl:DatatypeProperty ;
	rdfs:label "Flow Direction"@en .

uml:Flow_Direction-Shape
	rdf:type sh:PropertyShape ;
	sh:path uml:Flow_Direction ;
	sh:maxCount "1" ;
	sh:datatype xsd:string ;
	sh:maxLength "32" .

SpecIF:Revision
	rdf:type owl:DatatypeProperty ;
	rdfs:label "Revision"@en ;
	rdfs:label "Revision"@de ;
	rdfs:label "Révision"@fr .

SpecIF:Revision-Shape
	rdf:type sh:PropertyShape ;
	sh:path SpecIF:Revision ;
	sh:maxCount "1" ;
	sh:datatype xsd:string ;
	sh:maxLength "32" .

SpecIF:EngineeringDiscipline
	rdf:type owl:ObjectProperty ;
	rdfs:label "Engineering Discipline"@en ;
	rdfs:label "Ingenieurdisziplin"@de ;
	rdfs:label "Discipline d'ingénierie"@fr ;
	rdfs:comment "The engineering discipline involved by a development artefact."@en ;
	rdfs:range SpecIF:EngineeringDiscipline-Value .

SpecIF:EngineeringDiscipline-Shape
	rdf:type sh:PropertyShape ;
	sh:path SpecIF:EngineeringDiscipline ;
	sh:class SpecIF:EngineeringDiscipline-Value .

SpecIF:StakeholderGroup
	rdf:type owl:ObjectProperty ;
	rdfs:label "Stakeholder Group"@en ;
	rdfs:comment "Enumerated values for the 'Stakehoder Group' addressed by the term."@en ;
	rdfs:range SpecIF:StakeholderGroup-Value .

SpecIF:StakeholderGroup-Shape
	rdf:type sh:PropertyShape ;
	sh:path SpecIF:StakeholderGroup ;
	sh:maxCount "1" ;
	sh:class SpecIF:StakeholderGroup-Value .

SpecIF:Instantiation
	rdf:type owl:ObjectProperty ;
	rdfs:label "Instantiation" ;
	rdfs:comment "Indicates whether an instance of the class is created automatically, manually or both. Manual *and* automatic instantiation is allowed, if the property is omitted. The class is abstract and cannot be instantiated, if the property list is present, but empty.- 'user': a user creates, updates and deletes a resource's or statement's instance manually.- 'auto': a resource's or statement's instance is created, updated or deleted by an algorithm.- 'never': the class is abstract and cannot be instantiated." ;
	rdfs:range SpecIF:Instantiation-Value .

SpecIF:Instantiation-Shape
	rdf:type sh:PropertyShape ;
	sh:path SpecIF:Instantiation ;
	sh:class SpecIF:Instantiation-Value .

SpecIF:FitCriteria
	rdf:type owl:DatatypeProperty ;
	rdfs:label "Fit Criteria"@en ;
	rdfs:label "Abnahme-Kriterien"@de ;
	rdfs:label "Critères d'acceptation"@fr .

SpecIF:FitCriteria-Shape
	rdf:type sh:PropertyShape ;
	sh:path SpecIF:FitCriteria ;
	sh:maxCount "1" ;
	sh:datatype xsd:string .

dcterms:type
	rdf:type owl:DatatypeProperty ;
	rdfs:label "Element Type"@en ;
	rdfs:label "Element-Typ"@de ;
	rdfs:label "Type d'élément"@fr ;
	rdfs:comment "<p>The nature or genre of the resource. <small>(<i>source: <a href=\"http://purl.org/dc/elements/1.1/type\">DCMI</a></i>)</small></p><p>Recommended best practice is to use a controlled vocabulary such as the DCMI Type Vocabulary [DCMITYPE]. To describe the file format, physical medium, or dimensions of the resource, use the Format element.</p><p>For example, a [[FMC:Actor]] may represent a <i>System Function</i>, a <i>System Component</i> or a <i>User Role</i>. Similarly, in the context of process modelling, a FMC:Actor may represent a <i>Process Step</i> or again a <i>User Role</i>. So, all of these are meaningful values for a FMC:Actor's property named dcterms:type.</p>"@en .

dcterms:type-Shape
	rdf:type sh:PropertyShape ;
	sh:path dcterms:type ;
	sh:maxCount "1" ;
	sh:datatype xsd:string ;
	sh:maxLength "32" .

SpecIF:Icon
	rdf:type owl:DatatypeProperty ;
	rdfs:label "Icon"@en ;
	rdfs:label "Symbol"@de ;
	rdfs:label "Symbole"@fr ;
	rdfs:comment "A symbol or icon for display as a prefix to titles; applicable to all instances of the class. Is usually a XML-encoded UTF-8 symbol, can be an URL or dataURL."@en .

SpecIF:Icon-Shape
	rdf:type sh:PropertyShape ;
	sh:path SpecIF:Icon ;
	sh:maxCount "1" ;
	sh:datatype xsd:string ;
	sh:maxLength "256" .

SpecIF:LifecycleStatus
	rdf:type owl:ObjectProperty ;
	rdfs:label "Lifecycle"@en ;
	rdfs:label "Lebenszyklus"@de ;
	rdfs:label "Cycle de vie"@fr ;
	rdfs:comment "The 'Lifecycle Status' of the resource."@en ;
	rdfs:comment "Der 'Lebenszyklusstatus' der Ressource."@de ;
	rdfs:comment "L'état du cycle de vie de la ressource."@fr ;
	rdfs:range SpecIF:LifecycleStatus-Value .

SpecIF:LifecycleStatus-Shape
	rdf:type sh:PropertyShape ;
	sh:path SpecIF:LifecycleStatus ;
	sh:maxCount "1" ;
	sh:class SpecIF:LifecycleStatus-Value .

SpecIF:Priority
	rdf:type owl:ObjectProperty ;
	rdfs:label "Priority"@en ;
	rdfs:label "Priorität"@de ;
	rdfs:label "Priorité"@fr ;
	rdfs:comment "Enumerated values for the 'Priority' of the resource."@en ;
	rdfs:range SpecIF:Priority-Value .

SpecIF:Priority-Shape
	rdf:type sh:PropertyShape ;
	sh:path SpecIF:Priority ;
	sh:maxCount "1" ;
	sh:class SpecIF:Priority-Value .

IREB:RequirementType
	rdf:type owl:ObjectProperty ;
	rdfs:label "Type"@en ;
	rdfs:label "Art"@de ;
	rdfs:comment "According to the IREB, requirements are typically classified into functional requirements ([[IREB:FunctionalRequirement]]), quality requirements ([[IREB:QualityRequirement]]) and constraints ([[IREB:Constraint]]). The latter two are also called non-functional requirements."@en ;
	rdfs:comment "Nach dem IREB werden Anforderungen üblicherweise nach 'Art' in funktionale Anforderungen ([[IREB:FunctionalRequirement]]), Qualitätsanforderungen ([[IREB:QualityRequirement]]) und Randbedingungen ([[IREB:Constraint]]) unterteilt. Die beiden letzteren werden auch nicht-funktionale Anforderungen genannt."@de ;
	rdfs:comment "Selon l'IREB, les exigences sont généralement classées en exigences fonctionnelles ([[IREB:FunctionalRequirement]]), en exigences de qualité ([[IREB:QualityRequirement]]) et en contraintes ([[IREB:Constraint]]). Ces deux dernières sont également appelées exigences non fonctionnelles."@fr ;
	rdfs:range IREB:RequirementType-Value .

IREB:RequirementType-Shape
	rdf:type sh:PropertyShape ;
	sh:path IREB:RequirementType ;
	sh:maxCount "1" ;
	sh:class IREB:RequirementType-Value .

SpecIF:Probability
	rdf:type owl:DatatypeProperty ;
	rdfs:label "Probability"@en ;
	rdfs:label "Wahrscheinlichkeit"@de ;
	rdfs:label "Probabilité"@fr .

SpecIF:Probability-Shape
	rdf:type sh:PropertyShape ;
	sh:path SpecIF:Probability ;
	sh:maxCount "1" ;
	sh:datatype xsd:double ;
	sh:minInclusive "0" ;
	sh:maxInclusive "1" .

SpecIF:Impact
	rdf:type owl:DatatypeProperty ;
	rdfs:label "Impact"@en ;
	rdfs:label "Auswirkung"@de .

SpecIF:Impact-Shape
	rdf:type sh:PropertyShape ;
	sh:path SpecIF:Impact ;
	sh:maxCount "1" ;
	sh:datatype xsd:double ;
	sh:minInclusive "0" .

SpecIF:ModelFile
	rdf:type owl:DatatypeProperty ;
	rdfs:label "Model File"@en ;
	rdfs:comment "A file with partial model information."@en .

SpecIF:ModelFile-Shape
	rdf:type sh:PropertyShape ;
	sh:path SpecIF:ModelFile ;
	sh:maxCount "1" ;
	sh:datatype xsd:string ;
	sh:maxLength "256" .

ReqIF-WF:SupplierStatus
	rdf:type owl:ObjectProperty ;
	rdfs:label "Supplier Status"@en ;
	rdfs:label "Zustand Lieferant"@de ;
	rdfs:label "Statut coté Fournisseur"@fr ;
	rdfs:range ReqIF-WF:SupplierStatus-Value .

ReqIF-WF:SupplierStatus-Shape
	rdf:type sh:PropertyShape ;
	sh:path ReqIF-WF:SupplierStatus ;
	sh:maxCount "1" ;
	sh:class ReqIF-WF:SupplierStatus-Value .

ReqIF-WF:SupplierComment
	rdf:type owl:DatatypeProperty ;
	rdfs:label "Supplier Comment"@en ;
	rdfs:label "Kommentar Lieferant"@de ;
	rdfs:label "Commentaire du Client"@fr .

ReqIF-WF:SupplierComment-Shape
	rdf:type sh:PropertyShape ;
	sh:path ReqIF-WF:SupplierComment ;
	sh:datatype xsd:string .

ReqIF-WF:CustomerStatus
	rdf:type owl:ObjectProperty ;
	rdfs:label "Customer Status"@en ;
	rdfs:label "Zustand Kunde"@de ;
	rdfs:label "Statut coté Client"@fr ;
	rdfs:range ReqIF-WF:CustomerStatus-Value .

ReqIF-WF:CustomerStatus-Shape
	rdf:type sh:PropertyShape ;
	sh:path ReqIF-WF:CustomerStatus ;
	sh:maxCount "1" ;
	sh:class ReqIF-WF:CustomerStatus-Value .

ReqIF-WF:CustomerComment
	rdf:type owl:DatatypeProperty ;
	rdfs:label "Customer Comment"@en ;
	rdfs:label "Kommentar Kunde"@de ;
	rdfs:label "Commentaire du Client"@fr .

ReqIF-WF:CustomerComment-Shape
	rdf:type sh:PropertyShape ;
	sh:path ReqIF-WF:CustomerComment ;
	sh:datatype xsd:string .

#################################################################
# Ontology - Entity Classes
#################################################################

SpecIF:Paragraph
	rdfs:subClassOf pig:Entity ;
	rdfs:label "Paragraph"@en ;
	rdfs:label "Textabsatz"@de ;
	rdfs:label "Paragraphe"@fr ;
	rdfs:comment "<p>A 'Paragraph' is an unspecified information in a document at any level.</p>"@en ;
	rdfs:comment "<p>Ein 'Textabschnitt' in einem Dokument auf beliebiger Ebene.</p>"@de ;
	dcterms:modified "2024-03-02T20:55:23.295Z" .

SpecIF:Paragraph-Shape
	sh:targetClass SpecIF:Paragraph ;
	sh:property rdfs:label-Shape ;
	sh:property rdfs:comment-Shape ;
	sh:property SpecIF:Diagram-Shape ;
	sh:property dcterms:type-Shape .

pig:Hierarchy
	rdfs:subClassOf pig:Organizer ;
	rdfs:label "Hierarchy" ;
	rdfs:comment "A tree-shaped structure whose nodes reference a [[pig:Entity]] each. Specializations are among others [[pig:Outline]] (a document outline) and [[pig:BillOfMaterials]]. While a graph does not have a start nor an end, a hierarchy gives easy access to relevant content depending on the target group or purpose." ;
	dcterms:modified "2025-08-26T05:38:02.862Z" .

pig:Hierarchy-Shape
	sh:targetClass pig:Hierarchy ;
	sh:property rdfs:label-Shape ;
	sh:property rdfs:comment-Shape ;
	sh:property SpecIF:Icon-Shape ;
	sh:property dcterms:type-Shape ;
	sh:property SpecIF:LifecycleStatus-Shape .

SpecIF:ModelElement
	rdfs:subClassOf pig:Entity ;
	rdfs:label "Model Element"@en ;
	rdfs:label "Modellelement"@de ;
	rdfs:comment "Is a generalized type for model elements."@en ;
	rdfs:comment "Ist ein generalisierter Typ für Modellelemente."@de ;
	pig:Icon "&#x2606;" ;
	dcterms:modified "2025-03-08T20:23:37.245Z" .

SpecIF:ModelElement-Shape
	sh:targetClass SpecIF:ModelElement ;
	sh:property rdfs:label-Shape ;
	sh:property rdfs:comment-Shape ;
	sh:property dcterms:type-Shape .

SpecIF:Views
	rdfs:subClassOf pig:Hierarchy ;
	rdfs:label "Views"@en ;
	rdfs:label "Ansichten"@de ;
	dcterms:modified "2025-08-24T15:56:54.056Z" .

SpecIF:Views-Shape
	sh:targetClass SpecIF:Views ;
	sh:property rdfs:label-Shape ;
	sh:property rdfs:comment-Shape ;
	sh:property SpecIF:Icon-Shape ;
	sh:property dcterms:type-Shape ;
	sh:property SpecIF:LifecycleStatus-Shape .

pig:View
	rdfs:subClassOf pig:Organizer ;
	rdfs:label "View" ;
	rdfs:comment "A PIG organizer class representing a diagram with certain model-elements for a given communication purpose." ;
	dcterms:modified "2025-09-05T14:22:58.768Z" .

pig:View-Shape
	sh:targetClass pig:View ;
	sh:property rdfs:label-Shape ;
	sh:property rdfs:comment-Shape ;
	sh:property SpecIF:Icon-Shape ;
	sh:property dcterms:type-Shape ;
	sh:property SpecIF:Notation-Shape .

FMC:Actor
	rdfs:subClassOf SpecIF:ModelElement ;
	rdfs:label "Actor"@en ;
	rdfs:label "Akteur"@de ;
	rdfs:label "Acteur"@fr ;
	rdfs:comment "<p>An 'Actor' is a fundamental model element type representing an active entity, be it an activity, a process step, a function, a system component or a role.</p><p>The  particular use or original type is specified with a [[dcterms:type]] property of the 'FMC:Actor'. A value of that property should be an ontology-term, such as [[bpmn:processStep]].</p>"@en ;
	rdfs:comment "<p>Ein 'Akteur' ist ein fundamentaler Modellelementtyp, der eine aktive Entität darstellt, sei es eine Aktivität, ein Prozessschritt, eine Funktion, eine Systemkomponente oder eine Rolle.</p><p>Die spezielle Verwendung oder der ursprüngliche Typ wird mit einer [[dcterms:type]] Eigenschaft von 'FMC:Actor' spezifiziert. Die Werte dieser Eigenschaft können Ontologiebegriffe sein, wie z.B. [[bpmn:timer]].</p>"@de ;
	rdfs:comment "<p>Un 'Acteur' est un type d'élément de modèle fondamental représentant une entité active, qu'il s'agisse d'une activité, d'une étape de processus, d'une fonction, d'un composant de système ou d'un rôle.</p><p>L'utilisation particulière ou le type original est spécifié avec une propriété [[dcterms:type]] de 'FMC:Actor'. Les valeurs de cette propriété peuvent être des termes d'ontologie, tels que [[bpmn:timer]].</p>"@fr ;
	pig:Icon "&#x25A1;" ;
	dcterms:modified "2025-03-08T20:21:05.195Z" .

FMC:Actor-Shape
	sh:targetClass FMC:Actor ;
	sh:property rdfs:label-Shape ;
	sh:property rdfs:comment-Shape ;
	sh:property dcterms:type-Shape .

SpecIF:Collection
	rdfs:subClassOf SpecIF:ModelElement ;
	rdfs:label "Collection or Group"@en ;
	rdfs:label "Kollektion oder Gruppe"@de ;
	rdfs:label "Collection ou Groupe"@fr ;
	rdfs:comment "<p>A 'Collection' is a logical (often conceptual) group of resources linked with a [[SpecIF:contains]] statement. It corresponds to a <a href=\"https://camunda.com/bpmn/reference/\">'Group'</a> in BPMN Diagrams.</p><p>BPMN: An arbitrary set of objects can be defined as a Group to show that they logically belong together. <small>(<i>source: <a href=\"http://www.bpmn-tool.com/en/tutorial/\">BPMN Tutorial</a></i>)</small></p>"@en ;
	rdfs:comment "<p>Eine 'Kollektion' ist eine logische Gruppierung bestimmter Modellelemente, die per [[SpecIF:contains]] Relation zusammen gefasst sind. Sie entspricht einer <a href=\"https://camunda.com/bpmn/reference/\">'Gruppe'</a> in BPMN Diagrammen. <small>(<i>source: <a href=\"http://www.bpmn-tool.com/en/tutorial/\">BPMN Tutorial</a></i>)</small></p>"@de ;
	rdfs:comment "<p>Une 'collection' est un groupe logique (souvent conceptuel) de ressources liées par une déclaration [[SpecIF:contains]]. Elle correspond à un <a href=\"https://camunda.com/bpmn/reference/\">'groupe'</a> dans les diagrammes BPMN. <small>(<i>source: <a href=\"http://www.bpmn-tool.com/en/tutorial/\">BPMN Tutoriel</a></i>)</small></p>"@fr ;
	pig:Icon "⬚" ;
	dcterms:modified "2024-06-09T18:27:41.176Z" .

SpecIF:Collection-Shape
	sh:targetClass SpecIF:Collection ;
	sh:property rdfs:label-Shape ;
	sh:property rdfs:comment-Shape ;
	sh:property dcterms:type-Shape .

FMC:State
	rdfs:subClassOf SpecIF:ModelElement ;
	rdfs:label "State"@en ;
	rdfs:label "Zustand"@de ;
	rdfs:label "État"@fr ;
	rdfs:comment "<p>A 'State' is a fundamental model element type representing a passive entity, be it a value, a condition, an information storage or even a physical shape.</p><p>The particular use or the original type is specified with a [[dcterms:type]] property of the 'FMC:State'. A value of that property should bean  ontology-term, such as [[bpmn:dataObject]].</p>"@en ;
	rdfs:comment "<p>Ein 'Zustand' ist ein fundamentaler Modellelementtyp, der eine passive Entität darstellt, sei es ein Wert, ein Dokument, ein Informationsspeicher, eine Bedingung oder eine physische Beschaffenheit.</p><p>Die spezielle Verwendung oder der ursprüngliche Typ wird mit einer [[dcterms:type]] Eigenschaft von 'FMC:State' spezifiziert. Die Werte dieser Eigenschaft können Ontologiebegriffe sein, wie z.B. [[ArchiMate:DataObject]].</p>"@de ;
	rdfs:comment "<p>Un 'État' est un type d'élément de modèle fondamental représentant une entité passive, qu'il s'agisse d'une valeur, d'une condition, d'un stockage d'informations ou même d'une forme physique.</p><p>L'utilisation particulière ou le type original est spécifié avec une propriété [[dcterms:type]] de 'FMC:State'. Les valeurs de cette propriété peuvent être des termes d'ontologie, tels que [[ArchiMate:DataObject]].</p>"@fr ;
	pig:Icon "&#x25CB;" ;
	dcterms:modified "2025-03-08T20:04:01.555Z" .

FMC:State-Shape
	sh:targetClass FMC:State ;
	sh:property rdfs:label-Shape ;
	sh:property rdfs:comment-Shape ;
	sh:property dcterms:type-Shape .

FMC:Event
	rdfs:subClassOf SpecIF:ModelElement ;
	rdfs:label "Event"@en ;
	rdfs:label "Ereignis"@de ;
	rdfs:label "Évenement"@fr ;
	rdfs:comment "<p>An 'Event' is a fundamental model element type representing a time reference, a change in condition/value or more generally a synchronization primitive.</p><p>The particular use or the original type is specified with a [[dcterms:type]] property of the 'FMC:Event'. A value of that property should be an ontology-term, such as [[bpmn:startEvent]].</p>"@en ;
	rdfs:comment "<p>Ein 'Ereignis' ist ein fundamentaler Modellelementtyp, der eine Zeitreferenz, eine Änderung einer Bedingung/eines Wertes oder allgemeiner ein Synchronisationsmittel darstellt.</p><p>Die spezielle Verwendung oder der ursprüngliche Typ wird mit einer [[dcterms:type]] Eigenschaft von 'FMC:Event' spezifiziert. Die Werte dieser Eigenschaft sollen Ontologiebegriffe sein, wie z.B. [[bpmn:startEvent]].</p>"@de ;
	rdfs:comment "<p>Un 'Événement' est un type d'élément de modèle fondamental représentant une référence temporelle, un changement de condition/valeur ou plus généralement une primitive de synchronisation.</p><p>L'utilisation particulière ou le type original est spécifié avec une propriété [[dcterms:type]] de 'FMC:Event'. Les valeurs de cette propriété peuvent être des termes d'ontologie, tels que [[bpmn:startEvent]].</p>"@fr ;
	pig:Icon "&#x2662;" ;
	dcterms:modified "2025-03-08T19:57:15.384Z" .

FMC:Event-Shape
	sh:targetClass FMC:Event ;
	sh:property rdfs:label-Shape ;
	sh:property rdfs:comment-Shape ;
	sh:property dcterms:type-Shape .

schema:Role
	rdfs:subClassOf SpecIF:Paragraph ;
	rdfs:label "Role" ;
	rdfs:comment "Represents additional information about a relationship or property. For example a Role can be used to say that a &#39;member&#39; role linking some SportsTeam to a player occurred during a particular time period. Or that a Person&#39;s &#39;actor&#39; role in a Movie was for some particular characterName. Such properties can be attached to a Role entity, which is then associated with the main entities using ordinary properties like &#39;member&#39; or &#39;actor&#39;." ;
	dcterms:modified "2025-06-17T07:55:08.189Z" .

schema:Role-Shape
	sh:targetClass schema:Role ;
	sh:property rdfs:label-Shape ;
	sh:property rdfs:comment-Shape ;
	sh:property SpecIF:Diagram-Shape ;
	sh:property dcterms:type-Shape .

SpecIF:UserRole
	rdfs:subClassOf schema:Role ;
	rdfs:label "User Role"@en ;
	rdfs:label "Nutzerrolle"@de ;
	rdfs:label "Rôle utilisateur"@fr ;
	rdfs:comment "<p>This is a subclass of [[FMC:Actor]]; more precisely a value of it's property [[dcterms:type]].</p>" ;
	dcterms:modified "2025-09-06T15:29:44.104Z" .

SpecIF:UserRole-Shape
	sh:targetClass SpecIF:UserRole ;
	sh:property rdfs:label-Shape ;
	sh:property rdfs:comment-Shape ;
	sh:property SpecIF:Diagram-Shape ;
	sh:property dcterms:type-Shape .

SpecIF:Heading
	rdfs:subClassOf SpecIF:Paragraph ;
	rdfs:label "Heading"@en ;
	rdfs:label "Überschrift"@de ;
	rdfs:label "Intitulé"@fr ;
	rdfs:comment "A 'Heading' is a chapter title at any level with optional description."@en ;
	rdfs:comment "Eine 'Überschrift' in einem Dokument ist der Titel eines Kapitels. Sie kann eine Beschreibung haben, die als Einleitung oder Zusammenfassung des Kapitels genutzt werden kann."@de ;
	dcterms:modified "2024-03-02T15:28:50.414Z" .

SpecIF:Heading-Shape
	sh:targetClass SpecIF:Heading ;
	sh:property rdfs:label-Shape ;
	sh:property rdfs:comment-Shape ;
	sh:property SpecIF:Diagram-Shape ;
	sh:property dcterms:type-Shape .

IREB:Requirement
	rdfs:subClassOf SpecIF:Paragraph ;
	rdfs:label "Requirement"@en ;
	rdfs:label "Anforderung"@de ;
	rdfs:label "Exigence"@fr ;
	rdfs:comment "<p>A 'Requirement' is a singular documented physical and functional need that a particular design, product or process must be able to perform. <small>(<i>source: <a href=\"https://en.wikipedia.org/wiki/Requirement\">Wikipedia</a></i>)</small></p><p>Definition:</p><ol><li>A condition or capability needed by a user to solve a problem or achieve an objective.</li><li>A condition or capability that must be met or possessed by a system or system component to satisfy a contract, standard, specification, or other formally imposed documents.</li><li>A documented representation of a condition or capability as in (1) or (2).</li></ol><p>Note: The definition above is the classic one from IEEE Std 610.12 of 1990. Alternatively, we also give a more modern definition:</p><ol><li>A need perceived by a stakeholder.</li><li>A capability or property that a system shall have.</li><li>A documented representation of a need, capability or property.</li></ol>"@en ;
	rdfs:comment "<p>Eine 'Anforderung' ist ein einzelnes dokumentiertes physisches und funktionales Bedürfnis, das ein bestimmter Entwurf, ein Produkt oder ein Prozess erfüllen muss. <small>(<i>source: <a href=\"https://en.wikipedia.org/wiki/Requirement\">Wikipedia</a></i>)</small></p><p>Definition:</p><ol><li>Eine Bedingung oder Fähigkeit, die ein Benutzer benötigt, um ein Problem zu lösen oder ein Ziel zu erreichen.</li><li>Eine Bedingung oder Fähigkeit, die ein System oder eine Systemkomponente erfüllen oder besitzen muss, um einen Vertrag, eine Norm, eine Spezifikation oder ein anderes formal vorgeschriebenes Dokument zu erfüllen.</li><li>Eine dokumentierte Darstellung einer Bedingung oder Fähigkeit wie in (1) oder (2).</li></ol><p>Anmerkung: Die obige Definition ist die klassische Definition aus IEEE Std 610.12 von 1990. Alternativ geben wir auch eine modernere Definition an:</p><ol><li>Ein von einem Stakeholder wahrgenommener Bedarf.</li><li>Eine Fähigkeit oder Eigenschaft, die ein System haben soll.</li><li>Eine dokumentierte Darstellung eines Bedarfs, einer Fähigkeit oder Eigenschaft.</li></ol>"@de ;
	rdfs:comment "<p>Une 'Exigence' est un besoin physique et fonctionnel unique et documenté qu'une conception, un produit ou un processus particulier doit pouvoir satisfaire. <small>(<i>source: <a href=\"https://en.wikipedia.org/wiki/Requirement\">Wikipedia</a></i>)</small></p><p>Définition:</p><ol><li>Condition ou capacité dont un utilisateur a besoin pour résoudre un problème ou atteindre un objectif.</li><li>Condition ou capacité qui doit être remplie ou possédée par un système ou un composant de système pour satisfaire à un contrat, à une norme, à une spécification ou à d'autres documents imposés officiellement.</li><li>Une représentation documentée d'une condition ou d'une capacité comme dans (1) ou (2).</li></ol><p>Remarque: La définition ci-dessus est la définition classique de la norme IEEE 610.12 de 1990. Nous donnons également une définition plus moderne:</p><ol><li>Un besoin perçu par une partie prenante;</li><li>Une capacité ou une propriété qu'un système doit avoir.</li><li>Une représentation documentée d'un besoin, d'une capacité ou d'une propriété.</li></ol>"@fr ;
	pig:Icon "&#8623;" ;
	dcterms:modified "2023-04-01T14:10:11.167Z" .

IREB:Requirement-Shape
	sh:targetClass IREB:Requirement ;
	sh:property rdfs:label-Shape ;
	sh:property rdfs:comment-Shape ;
	sh:property SpecIF:Diagram-Shape ;
	sh:property dcterms:type-Shape ;
	sh:property SpecIF:Priority-Shape ;
	sh:property IREB:RequirementType-Shape ;
	sh:property SpecIF:StakeholderGroup-Shape .

DDP:ProductFunction
	rdfs:subClassOf SpecIF:ModelElement ;
	rdfs:label "Product Function" ;
	rdfs:comment "A product function describes the way a system works or performs a specific task."@en ;
	rdfs:comment "Eine Produktfunktion beschreibt die Art und Weise, wie ein System arbeitet oder eine bestimmte Aufgabe ausführt."@de ;
	dcterms:modified "2025-08-15T14:46:59.971Z" .

DDP:ProductFunction-Shape
	sh:targetClass DDP:ProductFunction ;
	sh:property rdfs:label-Shape ;
	sh:property rdfs:comment-Shape ;
	sh:property dcterms:type-Shape .

DDP:SystemComponent
	rdfs:subClassOf SpecIF:ModelElement ;
	rdfs:label "System Component" ;
	rdfs:comment "Represents a generic component of a system."@en ;
	rdfs:comment "Repräsentiert eine generische Systemkomponente."@de ;
	dcterms:modified "2025-08-15T14:47:23.918Z" .

DDP:SystemComponent-Shape
	sh:targetClass DDP:SystemComponent ;
	sh:property rdfs:label-Shape ;
	sh:property rdfs:comment-Shape ;
	sh:property dcterms:type-Shape .

DDP:ComponentInterface
	rdfs:subClassOf SpecIF:ModelElement ;
	rdfs:label "Component Interface" ;
	rdfs:comment "Represents a generic interface of a system component."@en ;
	rdfs:comment "Repräsentiert eine generische Schnittstelle einer Systemkomponente."@de ;
	dcterms:modified "2025-08-15T14:47:33.470Z" .

DDP:ComponentInterface-Shape
	sh:targetClass DDP:ComponentInterface ;
	sh:property rdfs:label-Shape ;
	sh:property rdfs:comment-Shape ;
	sh:property dcterms:type-Shape .

SpecIF:Comment
	rdfs:subClassOf pig:Entity ;
	rdfs:label "Comment"@en ;
	rdfs:label "Kommentar"@de ;
	rdfs:label "Commentaire"@fr ;
	rdfs:comment "A 'Comment' is reader feedback referring to a model element ('resource' or 'statement' in general)."@en ;
	pig:Icon "🗅" ;
	dcterms:modified "2024-03-09T16:59:44.361Z" .

SpecIF:Comment-Shape
	sh:targetClass SpecIF:Comment ;
	sh:property rdfs:comment-Shape .

SpecIF:Note
	rdfs:subClassOf SpecIF:Paragraph ;
	rdfs:label "Note" ;
	rdfs:comment "<p>A 'Note' is additional information by the author referring to any resource.</p>" ;
	dcterms:modified "2025-06-17T07:51:20.290Z" .

SpecIF:Note-Shape
	sh:targetClass SpecIF:Note ;
	sh:property rdfs:label-Shape ;
	sh:property rdfs:comment-Shape ;
	sh:property SpecIF:Diagram-Shape ;
	sh:property dcterms:type-Shape .

SpecIF:Permissions
	rdfs:subClassOf pig:Entity ;
	rdfs:label "Permission"@en ;
	rdfs:label "Berechtigung"@de ;
	rdfs:comment "Permissions are a set of user rights, each allowing to use a certain function and/or to access a certain data set."@en ;
	dcterms:modified "2024-04-12T10:32:51.211Z" .

SpecIF:Permissions-Shape
	sh:targetClass SpecIF:Permissions ;
	sh:property rdfs:label-Shape .

IREB:Risk
	rdfs:subClassOf SpecIF:Paragraph ;
	rdfs:label "Risk" ;
	rdfs:comment "<p>An event that threatens the success of an endeavor, e.g., of developing or operating a system. A risk is typically assessed in terms of its probability and potential damage.</p>" ;
	dcterms:modified "2025-06-17T07:54:21.582Z" .

IREB:Risk-Shape
	sh:targetClass IREB:Risk ;
	sh:property rdfs:label-Shape ;
	sh:property rdfs:comment-Shape ;
	sh:property SpecIF:Diagram-Shape ;
	sh:property dcterms:type-Shape ;
	sh:property SpecIF:Probability-Shape ;
	sh:property SpecIF:Impact-Shape .

pig:HierarchyRoot
	rdfs:subClassOf pig:Organizer ;
	rdfs:label "Hierarchy Root"@en ;
	rdfs:comment "A node (vertex) in a graph anchoring all instances of [[pig:Hierarchy]]."@en ;
	dcterms:modified "2025-08-26T05:34:02.768Z" .

pig:HierarchyRoot-Shape
	sh:targetClass pig:HierarchyRoot ;
	sh:property rdfs:label-Shape ;
	sh:property rdfs:comment-Shape ;
	sh:property SpecIF:Icon-Shape ;
	sh:property dcterms:type-Shape .

pig:BillOfMaterials
	rdfs:subClassOf pig:Hierarchy ;
	rdfs:label "Bill of Materials" ;
	rdfs:comment "<p>A bill of materials or product structure (sometimes bill of material, BOM or associated list) is a list of the raw materials, sub-assemblies, intermediate assemblies, sub-components, parts and the quantities of each needed to manufacture an end product. A BOM may be used for communication between manufacturing partners, or confined to a single manufacturing plant. <small>(<i>source: <a href=\"https://en.wikipedia.org/wiki/Bill_of_materials\">Wikipedia</a></i>)</small></p>" ;
	dcterms:modified "2025-08-26T05:45:44.343Z" .

pig:BillOfMaterials-Shape
	sh:targetClass pig:BillOfMaterials ;
	sh:property rdfs:label-Shape ;
	sh:property rdfs:comment-Shape ;
	sh:property SpecIF:Icon-Shape ;
	sh:property dcterms:type-Shape ;
	sh:property SpecIF:LifecycleStatus-Shape .

SpecIF:BusinessProcesses
	rdfs:subClassOf SpecIF:Views ;
	rdfs:label "Business Processes" ;
	dcterms:modified "2025-06-17T07:57:34.078Z" .

SpecIF:BusinessProcesses-Shape
	sh:targetClass SpecIF:BusinessProcesses ;
	sh:property rdfs:label-Shape ;
	sh:property rdfs:comment-Shape ;
	sh:property SpecIF:Icon-Shape ;
	sh:property dcterms:type-Shape ;
	sh:property SpecIF:LifecycleStatus-Shape .

SpecIF:Glossary
	rdfs:subClassOf pig:Hierarchy ;
	rdfs:label "Model Elements (Glossary)" ;
	dcterms:modified "2025-06-17T07:57:50.341Z" .

SpecIF:Glossary-Shape
	sh:targetClass SpecIF:Glossary ;
	sh:property rdfs:label-Shape ;
	sh:property rdfs:comment-Shape ;
	sh:property SpecIF:Icon-Shape ;
	sh:property dcterms:type-Shape ;
	sh:property SpecIF:LifecycleStatus-Shape .

bpmn:Process
	rdfs:subClassOf pig:View ;
	rdfs:label "Business Process" ;
	dcterms:modified "2025-06-17T08:01:09.565Z" .

bpmn:Process-Shape
	sh:targetClass bpmn:Process ;
	sh:property rdfs:label-Shape ;
	sh:property rdfs:comment-Shape ;
	sh:property SpecIF:Icon-Shape ;
	sh:property dcterms:type-Shape ;
	sh:property SpecIF:Notation-Shape .

bpmn:Participant
	rdfs:subClassOf FMC:Actor ;
	rdfs:label "Participant" ;
	dcterms:modified "2025-06-17T08:01:18.141Z" .

bpmn:Participant-Shape
	sh:targetClass bpmn:Participant ;
	sh:property rdfs:label-Shape ;
	sh:property rdfs:comment-Shape ;
	sh:property dcterms:type-Shape .

uml:Package
	rdfs:subClassOf SpecIF:Collection ;
	rdfs:label "Package"@en ;
	dcterms:modified "2024-06-13T07:55:07.739Z" .

uml:Package-Shape
	sh:targetClass uml:Package ;
	sh:property rdfs:label-Shape ;
	sh:property rdfs:comment-Shape ;
	sh:property dcterms:type-Shape .

uml:Actor
	rdfs:subClassOf FMC:Actor ;
	rdfs:label "Actor"@en ;
	dcterms:modified "2023-09-12T06:33:15.885Z" .

uml:Actor-Shape
	sh:targetClass uml:Actor ;
	sh:property rdfs:label-Shape ;
	sh:property rdfs:comment-Shape ;
	sh:property dcterms:type-Shape .

uml:Port
	rdfs:subClassOf FMC:Actor ;
	rdfs:label "Port"@en ;
	rdfs:label "Schnittstelle"@de ;
	dcterms:modified "2024-07-09T05:29:06.284Z" .

uml:Port-Shape
	sh:targetClass uml:Port ;
	sh:property rdfs:label-Shape ;
	sh:property rdfs:comment-Shape ;
	sh:property dcterms:type-Shape ;
	sh:property uml:is_Service-Shape ;
	sh:property uml:Flow_Direction-Shape .

uml:StateMachine
	rdfs:subClassOf FMC:Actor ;
	rdfs:label "UML State Machine" ;
	dcterms:modified "2025-04-18T15:01:06.865Z" .

uml:StateMachine-Shape
	sh:targetClass uml:StateMachine ;
	sh:property rdfs:label-Shape ;
	sh:property rdfs:comment-Shape ;
	sh:property dcterms:type-Shape .

uml:UseCase
	rdfs:subClassOf FMC:Actor ;
	rdfs:label "Use Case" ;
	dcterms:modified "2025-06-28T12:29:38.963Z" .

uml:UseCase-Shape
	sh:targetClass uml:UseCase ;
	sh:property rdfs:label-Shape ;
	sh:property rdfs:comment-Shape ;
	sh:property dcterms:type-Shape .

uml:Activity
	rdfs:subClassOf FMC:Actor ;
	rdfs:label "UML Activity" ;
	dcterms:modified "2025-04-23T07:46:20.849Z" .

uml:Activity-Shape
	sh:targetClass uml:Activity ;
	sh:property rdfs:label-Shape ;
	sh:property rdfs:comment-Shape ;
	sh:property dcterms:type-Shape .

uml:Region
	rdfs:subClassOf FMC:Actor ;
	rdfs:label "UML Region" ;
	dcterms:modified "2025-04-23T07:46:59.562Z" .

uml:Region-Shape
	sh:targetClass uml:Region ;
	sh:property rdfs:label-Shape ;
	sh:property rdfs:comment-Shape ;
	sh:property dcterms:type-Shape .

uml:State
	rdfs:subClassOf FMC:State ;
	rdfs:label "UML State" ;
	dcterms:modified "2025-04-18T15:07:47.101Z" .

uml:State-Shape
	sh:targetClass uml:State ;
	sh:property rdfs:label-Shape ;
	sh:property rdfs:comment-Shape ;
	sh:property dcterms:type-Shape .

uml:Transition
	rdfs:subClassOf FMC:Actor ;
	rdfs:label "UML Transition" ;
	dcterms:modified "2025-04-23T07:46:41.649Z" .

uml:Transition-Shape
	sh:targetClass uml:Transition ;
	sh:property rdfs:label-Shape ;
	sh:property rdfs:comment-Shape ;
	sh:property dcterms:type-Shape .

uml:SignalEvent
	rdfs:subClassOf FMC:Event ;
	rdfs:label "Signal-Event" ;
	dcterms:modified "2025-04-22T09:28:25.620Z" .

uml:SignalEvent-Shape
	sh:targetClass uml:SignalEvent ;
	sh:property rdfs:label-Shape ;
	sh:property rdfs:comment-Shape ;
	sh:property dcterms:type-Shape .

uml:CallEvent
	rdfs:subClassOf FMC:Event ;
	rdfs:label "Call-Event" ;
	dcterms:modified "2025-04-22T09:29:19.849Z" .

uml:CallEvent-Shape
	sh:targetClass uml:CallEvent ;
	sh:property rdfs:label-Shape ;
	sh:property rdfs:comment-Shape ;
	sh:property dcterms:type-Shape .

uml:ChangeEvent
	rdfs:subClassOf FMC:Event ;
	rdfs:label "Change-Event" ;
	dcterms:modified "2025-04-22T09:30:14.449Z" .

uml:ChangeEvent-Shape
	sh:targetClass uml:ChangeEvent ;
	sh:property rdfs:label-Shape ;
	sh:property rdfs:comment-Shape ;
	sh:property dcterms:type-Shape .

uml:CallBehaviorAction
	rdfs:subClassOf FMC:Actor ;
	rdfs:label "UML Call Behavior Action" ;
	dcterms:modified "2025-04-23T13:55:20.312Z" .

uml:CallBehaviorAction-Shape
	sh:targetClass uml:CallBehaviorAction ;
	sh:property rdfs:label-Shape ;
	sh:property rdfs:comment-Shape ;
	sh:property dcterms:type-Shape .

uml:ActivityFinalNode
	rdfs:subClassOf FMC:Actor ;
	rdfs:label "UML Activity Final Node" ;
	dcterms:modified "2025-06-28T12:12:58.883Z" .

uml:ActivityFinalNode-Shape
	sh:targetClass uml:ActivityFinalNode ;
	sh:property rdfs:label-Shape ;
	sh:property rdfs:comment-Shape ;
	sh:property dcterms:type-Shape .

IREB:Stakeholder
	rdfs:subClassOf schema:Role ;
	rdfs:label "Stakeholder" ;
	rdfs:comment "<p>A person or organization that has a (direct or indirect) influence on a system’s requirements. Indirect influence also includes situations where a person or organization is impacted by the system.</p><p>This is a subclass of [[FMC:Actor]], more precisely a value of it's property [[dcterms:type]].</p>" ;
	dcterms:modified "2025-06-28T12:13:45.944Z" .

IREB:Stakeholder-Shape
	sh:targetClass IREB:Stakeholder ;
	sh:property rdfs:label-Shape ;
	sh:property rdfs:comment-Shape ;
	sh:property SpecIF:Diagram-Shape ;
	sh:property dcterms:type-Shape .

SpecIF:Reader
	rdfs:subClassOf SpecIF:UserRole ;
	rdfs:label "Reader"@en ;
	rdfs:label "Leser"@de ;
	dcterms:modified "2024-06-13T07:56:45.423Z" .

SpecIF:Reader-Shape
	sh:targetClass SpecIF:Reader ;
	sh:property rdfs:label-Shape ;
	sh:property rdfs:comment-Shape ;
	sh:property SpecIF:Diagram-Shape ;
	sh:property dcterms:type-Shape .

SpecIF:Editor
	rdfs:subClassOf SpecIF:UserRole ;
	rdfs:label "Editor"@en ;
	dcterms:modified "2024-06-13T07:56:57.045Z" .

SpecIF:Editor-Shape
	sh:targetClass SpecIF:Editor ;
	sh:property rdfs:label-Shape ;
	sh:property rdfs:comment-Shape ;
	sh:property SpecIF:Diagram-Shape ;
	sh:property dcterms:type-Shape .

SpecIF:Feature
	rdfs:subClassOf SpecIF:Paragraph ;
	rdfs:label "Feature"@en ;
	rdfs:label "Merkmal"@de ;
	rdfs:label "Caractéristique"@fr ;
	rdfs:comment "<p>A 'Feature' is an intentional distinguishing characteristic of a system, often a unique selling proposition.</p>"@en ;
	rdfs:comment "Ein 'Merkmal' ist eine geplante Eigenschaft oder Funktion eines Systems, oft ein Alleinstellungsmerkmal zur Stärkung der Wettbewerbsposition."@de ;
	rdfs:comment "Une 'Caractéristique' est un trait distinctif intentionnel d'un système, souvent une proposition de vente unique."@fr ;
	pig:Icon "✶" ;
	dcterms:modified "2023-07-16T09:48:41.722Z" .

SpecIF:Feature-Shape
	sh:targetClass SpecIF:Feature ;
	sh:property rdfs:label-Shape ;
	sh:property rdfs:comment-Shape ;
	sh:property SpecIF:Diagram-Shape ;
	sh:property dcterms:type-Shape ;
	sh:property SpecIF:Priority-Shape .

SpecIF:UserStory
	rdfs:subClassOf SpecIF:Paragraph ;
	rdfs:label "User Story"@en ;
	rdfs:comment "<p>A user story is an informal, general explanation of a software feature written from the perspective of the end user. Its purpose is to articulate how a software feature will provide value to the customer.</p><p>This is a subclass of [[IREB:Requirement]], more precisely a value of it's property [[dcterms:type]].</p>"@en ;
	pig:Icon "&#x263A;" ;
	dcterms:modified "2024-06-13T07:53:56.470Z" .

SpecIF:UserStory-Shape
	sh:targetClass SpecIF:UserStory ;
	sh:property rdfs:label-Shape ;
	sh:property rdfs:comment-Shape ;
	sh:property SpecIF:Diagram-Shape ;
	sh:property dcterms:type-Shape ;
	sh:property SpecIF:Priority-Shape .

SpecIF:PainPoint
	rdfs:subClassOf SpecIF:Paragraph ;
	rdfs:label "Pain Point"@en ;
	rdfs:label "Schmerzpunkt"@de ;
	rdfs:comment "<p>A problem, frustration, or troublesome issue, especially one experienced by consumers, customers, or employees: Getting stuck in a slow checkout line is a major pain point for grocery shoppers.</p><p>This is a subclass of [[IREB:Requirement]], more precisely a value of it's property [[dcterms:type]].</p>"@en ;
	pig:Icon "&#x2702;" ;
	dcterms:modified "2024-06-13T07:54:07.654Z" .

SpecIF:PainPoint-Shape
	sh:targetClass SpecIF:PainPoint ;
	sh:property rdfs:label-Shape ;
	sh:property rdfs:comment-Shape ;
	sh:property SpecIF:Diagram-Shape ;
	sh:property dcterms:type-Shape .

ArchiMate:ApplicationComponent
	rdfs:subClassOf FMC:Actor ;
	rdfs:label "Application Component" ;
	rdfs:comment "Definition: An application component represents an encapsulation of application functionality aligned to implementation structure, which is modular and replaceable. It encapsulates its behavior and data, exposes services, and makes them available through interfaces.An application component is a self-contained unit. As such, it is independently deployable, re-usable, and replaceable. An application component performs one or more application functions. It encapsulates its contents: its functionality is only accessible through a set of application interfaces. Cooperating application components are connected via application collaborations.An application component may be assigned to one or more application functions. An application component has one or more application interfaces, which expose its functionality. Application interfaces of other application components may serve an application component. The name of an application component should preferably be a noun.The application component element is used to model entire applications (i.e., deployed and operational IT systems, as defined by the <a href=\"https://www.opengroup.org/bookstore/catalog/g116.htm\">TOGAF framework</a>) and individual parts of such applications, at all relevant levels of detail.<small>Source: <a href=\"https://pubs.opengroup.org/architecture/archimate30-doc/chap09.html\">ArchiMate® 3.0 Specification</a></small>"@en ;
	dcterms:modified "2025-06-17T07:43:29.700Z" .

ArchiMate:ApplicationComponent-Shape
	sh:targetClass ArchiMate:ApplicationComponent ;
	sh:property rdfs:label-Shape ;
	sh:property rdfs:comment-Shape ;
	sh:property dcterms:type-Shape .

ArchiMate:DataObject
	rdfs:subClassOf FMC:State ;
	rdfs:label "Data Object" ;
	rdfs:comment "Definition: A data object represents data structured for automated processing.A data object should be a self-contained piece of information with a clear meaning to the business, not just to the application level. Typical examples of data objects are a customer record, a client database, or an insurance claim.The ArchiMate language in general focuses on the modeling of types, not instances, since this is the most relevant at the Enterprise Architecture level of description. Hence a data object typically models an object type (cf. a UML class) of which multiple instances may exist in operational applications. An important exception is when a data object is used to model a data collection such as a database, of which only one instance exists.An application function or process can operate on data objects. A data object may be communicated via interactions and used or produced by application services. A data object can be accessed by an application function, application interaction, or application service. A data object may realize a business object, and may be realized by an artifact. A data object may have association, specialization, aggregation, or composition relationships with other data objects. The name of a data object should preferably be a noun.<small>Source: <a href=\"https://pubs.opengroup.org/architecture/archimate30-doc/chap09.html\">ArchiMate® 3.0 Specification</a></small>"@en ;
	dcterms:modified "2025-06-17T07:44:55.944Z" .

ArchiMate:DataObject-Shape
	sh:targetClass ArchiMate:DataObject ;
	sh:property rdfs:label-Shape ;
	sh:property rdfs:comment-Shape ;
	sh:property dcterms:type-Shape .

ArchiMate:BusinessObject
	rdfs:subClassOf FMC:State ;
	rdfs:label "Business Object" ;
	rdfs:comment "Definition: A business object represents a concept used within a particular business domain.The ArchiMate language in general focuses on the modeling of types, not instances, since this is the most relevant at the Enterprise Architecture level of description. Hence a business object typically models an object type (cf. a UML class) of which multiple instances may exist in operations. Only occasionally, business objects represent actual instances of information produced and consumed by behavior elements such as business processes. This is in particular the case for singleton types; i.e., types that have only one instance.A wide variety of types of business objects can be defined. Business objects are passive in the sense that they do not trigger or perform processes. A business object could be used to represent information assets that are relevant from a business point of view and can be realized by data objects.Business objects may be accessed (e.g., in the case of information objects, they may be created, read, written) by a business process, function, business interaction, business event, or business service. A business object may have association, specialization, aggregation, or composition relationships with other business objects. A business object may be realized by a representation or by a data object (or both). The name of a business object should preferably be a noun.<small>Source: <a href=\"https://pubs.opengroup.org/architecture/archimate30-doc/chap08.html\">ArchiMate® 3.0 Specification</a></small>"@en ;
	dcterms:modified "2025-06-17T07:45:08.525Z" .

ArchiMate:BusinessObject-Shape
	sh:targetClass ArchiMate:BusinessObject ;
	sh:property rdfs:label-Shape ;
	sh:property rdfs:comment-Shape ;
	sh:property dcterms:type-Shape .

DDP:Source
	rdfs:subClassOf SpecIF:Paragraph ;
	rdfs:label "Source File"@en ;
	rdfs:label "Quelldatei"@de ;
	rdfs:comment "A 'Source' is a file containing partial model information created by an authoring system."@en ;
	pig:Icon "🗎" ;
	dcterms:modified "2025-08-15T14:48:46.648Z" .

DDP:Source-Shape
	sh:targetClass DDP:Source ;
	sh:property rdfs:label-Shape ;
	sh:property rdfs:comment-Shape ;
	sh:property SpecIF:Diagram-Shape ;
	sh:property dcterms:type-Shape ;
	sh:property SpecIF:ModelFile-Shape .

pig:Package
	rdfs:subClassOf pig:Organizer ;
	rdfs:label "Package" ;
	rdfs:comment "A PIG organizer class comprising all information of a given package." ;
	dcterms:modified "2025-06-12T12:20:44.561Z" .

pig:Package-Shape
	sh:targetClass pig:Package ;
	sh:property rdfs:label-Shape ;
	sh:property rdfs:comment-Shape ;
	sh:property SpecIF:Icon-Shape ;
	sh:property dcterms:type-Shape .

pig:Product
	rdfs:subClassOf pig:Organizer ;
	rdfs:label "Product" ;
	rdfs:comment "A PIG organizer class comprising all information of a given product." ;
	dcterms:modified "2025-08-15T19:42:59.946Z" .

pig:Product-Shape
	sh:targetClass pig:Product ;
	sh:property rdfs:label-Shape ;
	sh:property rdfs:comment-Shape ;
	sh:property SpecIF:Icon-Shape ;
	sh:property dcterms:type-Shape .

pig:Outline
	rdfs:subClassOf pig:Organizer ;
	rdfs:label "Outline" ;
	rdfs:comment "A PIG organizer class comprising all information items of a human-readable document. As usual, the outline is hierarchically organized." ;
	dcterms:modified "2025-08-15T19:43:10.796Z" .

pig:Outline-Shape
	sh:targetClass pig:Outline ;
	sh:property rdfs:label-Shape ;
	sh:property rdfs:comment-Shape ;
	sh:property SpecIF:Icon-Shape ;
	sh:property dcterms:type-Shape .

ReqIF-WF:Requirement
	rdfs:subClassOf IREB:Requirement ;
	rdfs:label "Requirement (SRC)"@en ;
	rdfs:label "Anforderung (SRC)"@de ;
	rdfs:comment "<p>A 'Requirement' is a singular documented physical and functional need that a particular design, product or process must be able to perform.  <small>(<i>source: <a href=\"https://en.wikipedia.org/wiki/Requirement\">Wikipedia</a></i>)</small></p><p>Definition:</p><ol><li>A condition or capability needed by a user to solve a problem or achieve an objective.</li><li>A condition or capability that must be met or possessed by a system or system component to satisfy a contract, standard, specification, or other formally imposed documents.</li><li>A documented representation of a condition or capability as in (1) or (2).</li></ol><p>Note: The definition above is the classic one from IEEE Std 610.12 of 1990. Alternatively, we also give a more modern definition:</p><ol><li>A need perceived by a stakeholder.</li><li>A capability or property that a system shall have.</li><li>A documented representation of a need, capability or property.</li></ol>"@en ;
	pig:Icon "❢" ;
	dcterms:modified "2025-08-15T14:59:24.802Z" .

ReqIF-WF:Requirement-Shape
	sh:targetClass ReqIF-WF:Requirement ;
	sh:property rdfs:label-Shape ;
	sh:property rdfs:comment-Shape ;
	sh:property SpecIF:Diagram-Shape ;
	sh:property dcterms:type-Shape ;
	sh:property SpecIF:Priority-Shape ;
	sh:property IREB:RequirementType-Shape ;
	sh:property SpecIF:StakeholderGroup-Shape ;
	sh:property ReqIF-WF:SupplierStatus-Shape ;
	sh:property ReqIF-WF:SupplierComment-Shape ;
	sh:property ReqIF-WF:CustomerStatus-Shape ;
	sh:property ReqIF-WF:CustomerComment-Shape .

#################################################################
# Ontology - Relationship Classes
#################################################################

SpecIF:relates
	rdfs:subClassOf pig:Relationship ;
	rdfs:label "relates"@en ;
	rdfs:label "verbindet"@de ;
	rdfs:label "relie"@fr ;
	rdfs:comment "Is a generalized type for model relations."@en ;
	rdfs:comment "Ist ein generalisierter Typ für Modellrelationen."@de ;
	dcterms:modified "2024-06-09T12:35:33.150Z" .

SpecIF:relates-hasSource
	rdfs:subPropertyOf pig:eligibleSource ;
	rdfs:label "Connects the source of SpecIF:relates" ;
	rdfs:domain SpecIF:relates ;
	dcterms:modified "2024-06-09T12:35:33.150Z" .

SpecIF:relates-hasTarget
	rdfs:subPropertyOf pig:eligibleTarget ;
	rdfs:label "Connects the target of SpecIF:relates" ;
	rdfs:domain SpecIF:relates ;
	dcterms:modified "2024-06-09T12:35:33.150Z" .

SpecIF:relates-Shape
	sh:targetClass SpecIF:relates ;
	sh:property dcterms:type-Shape ;
	sh:property [ 
		sh:path SpecIF:relates-hasSource ;
		sh:minCount 1 ;
		sh:maxCount 1
	] ;
	sh:property [ 
		sh:path SpecIF:relates-hasTarget ;
		sh:minCount 1 ;
		sh:maxCount 1
	] .

dcterms:hasPart
	rdfs:subClassOf SpecIF:relates ;
	rdfs:label "has part"@en ;
	rdfs:label "enthält"@de ;
	rdfs:label "contient"@fr ;
	rdfs:comment "A related resource that is included either physically or logically in the described resource.*Comment: This property is intended to be used with non-literal values. This property is an inverse property of [[dcterms:isPartOf]].*"@en ;
	dcterms:modified "2024-06-18T12:23:12.163Z" .

dcterms:hasPart-hasSource
	rdfs:subPropertyOf pig:eligibleSource ;
	rdfs:label "Connects the source of dcterms:hasPart" ;
	rdfs:domain dcterms:hasPart ;
	rdfs:range [ owl:unionOf( FMC:Actor FMC:State SpecIF:Collection SpecIF:ModelElement )] ;
	dcterms:modified "2024-06-18T12:23:12.163Z" .

dcterms:hasPart-hasTarget
	rdfs:subPropertyOf pig:eligibleTarget ;
	rdfs:label "Connects the target of dcterms:hasPart" ;
	rdfs:domain dcterms:hasPart ;
	rdfs:range [ owl:unionOf( FMC:Actor FMC:State SpecIF:Collection SpecIF:ModelElement uml:Port )] ;
	dcterms:modified "2024-06-18T12:23:12.163Z" .

dcterms:hasPart-Shape
	sh:targetClass dcterms:hasPart ;
	sh:property dcterms:type-Shape ;
	sh:property [ 
		sh:path dcterms:hasPart-hasSource ;
		sh:class [ owl:unionOf( FMC:Actor FMC:State SpecIF:Collection SpecIF:ModelElement )] ;
		sh:minCount 1 ;
		sh:maxCount 1
	] ;
	sh:property [ 
		sh:path dcterms:hasPart-hasTarget ;
		sh:class [ owl:unionOf( FMC:Actor FMC:State SpecIF:Collection SpecIF:ModelElement uml:Port )] ;
		sh:minCount 1 ;
		sh:maxCount 1
	] .

SpecIF:handles
	rdfs:subClassOf pig:Relationship ;
	rdfs:label "handles"@en ;
	rdfs:label "befördert"@de ;
	rdfs:comment "<p>The relationship indicates that an element (represented by a [[FMC:Actor]]) provides or consumes material, energy or information (represented by a [[FMC:State]]).</p>"@en ;
	dcterms:modified "2024-07-14T12:58:29.336Z" .

SpecIF:handles-hasSource
	rdfs:subPropertyOf pig:eligibleSource ;
	rdfs:label "Connects the source of SpecIF:handles" ;
	rdfs:domain SpecIF:handles ;
	rdfs:range [ owl:unionOf( FMC:Actor uml:Port SpecIF:ModelElement )] ;
	dcterms:modified "2024-07-14T12:58:29.336Z" .

SpecIF:handles-hasTarget
	rdfs:subPropertyOf pig:eligibleTarget ;
	rdfs:label "Connects the target of SpecIF:handles" ;
	rdfs:domain SpecIF:handles ;
	rdfs:range [ owl:unionOf( FMC:State SpecIF:ModelElement )] ;
	dcterms:modified "2024-07-14T12:58:29.336Z" .

SpecIF:handles-Shape
	sh:targetClass SpecIF:handles ;
	sh:property [ 
		sh:path SpecIF:handles-hasSource ;
		sh:class [ owl:unionOf( FMC:Actor uml:Port SpecIF:ModelElement )] ;
		sh:minCount 1 ;
		sh:maxCount 1
	] ;
	sh:property [ 
		sh:path SpecIF:handles-hasTarget ;
		sh:class [ owl:unionOf( FMC:State SpecIF:ModelElement )] ;
		sh:minCount 1 ;
		sh:maxCount 1
	] .

SpecIF:accesses
	rdfs:subClassOf SpecIF:relates ;
	rdfs:label "accesses, stores"@en ;
	rdfs:label "schreibt und liest"@de ;
	rdfs:label "écrit et lit"@fr ;
	rdfs:comment "A [[FMC:Actor]] 'accesses' (writes and reads) a [[FMC:State]]."@en ;
	dcterms:modified "2024-07-14T12:32:07.132Z" .

SpecIF:accesses-hasSource
	rdfs:subPropertyOf pig:eligibleSource ;
	rdfs:label "Connects the source of SpecIF:accesses" ;
	rdfs:domain SpecIF:accesses ;
	rdfs:range [ owl:unionOf( FMC:Actor uml:Port )] ;
	dcterms:modified "2024-07-14T12:32:07.132Z" .

SpecIF:accesses-hasTarget
	rdfs:subPropertyOf pig:eligibleTarget ;
	rdfs:label "Connects the target of SpecIF:accesses" ;
	rdfs:domain SpecIF:accesses ;
	rdfs:range FMC:State ;
	dcterms:modified "2024-07-14T12:32:07.132Z" .

SpecIF:accesses-Shape
	sh:targetClass SpecIF:accesses ;
	sh:property dcterms:type-Shape ;
	sh:property [ 
		sh:path SpecIF:accesses-hasSource ;
		sh:class [ owl:unionOf( FMC:Actor uml:Port )] ;
		sh:minCount 1 ;
		sh:maxCount 1
	] ;
	sh:property [ 
		sh:path SpecIF:accesses-hasTarget ;
		sh:class FMC:State ;
		sh:minCount 1 ;
		sh:maxCount 1
	] .

ArchiMate:Uniting
	rdfs:subClassOf dcterms:hasPart ;
	rdfs:label "unites" ;
	rdfs:comment "General containment. In ArchiMate, the uniting concept includes:- The *composition* relationship represents that an element consists of one or more other concepts.- The *aggregation* relationship represents that an element combines one or more other concepts.- The *assignment* relationship represents the allocation of responsibility, performance of behavior, storage, or execution.- The *realization* relationship represents that an entity plays a critical role in the creation, achievement, sustenance, or operation of a more abstract entity.The kind of uniting is specified in a property with title [[dcterms:type]]."@en ;
	dcterms:modified "2025-09-06T14:52:36.710Z" .

ArchiMate:Uniting-hasSource
	rdfs:subPropertyOf pig:eligibleSource ;
	rdfs:label "Connects the source of ArchiMate:Uniting" ;
	rdfs:domain ArchiMate:Uniting ;
	dcterms:modified "2025-09-06T14:52:36.710Z" .

ArchiMate:Uniting-hasTarget
	rdfs:subPropertyOf pig:eligibleTarget ;
	rdfs:label "Connects the target of ArchiMate:Uniting" ;
	rdfs:domain ArchiMate:Uniting ;
	dcterms:modified "2025-09-06T14:52:36.710Z" .

ArchiMate:Uniting-Shape
	sh:targetClass ArchiMate:Uniting ;
	sh:property dcterms:type-Shape ;
	sh:property [ 
		sh:path ArchiMate:Uniting-hasSource ;
		sh:minCount 1 ;
		sh:maxCount 1
	] ;
	sh:property [ 
		sh:path ArchiMate:Uniting-hasTarget ;
		sh:minCount 1 ;
		sh:maxCount 1
	] .

FMC:communicatesWith
	rdfs:subClassOf pig:Relationship ;
	rdfs:label "communicates with"@en ;
	rdfs:label "kommuniziert mit"@de ;
	rdfs:label "communique avec"@fr ;
	rdfs:comment "A [[FMC:Actor]] 'communicates' with a [[FMC:Actor]]." ;
	dcterms:modified "2023-03-15T09:13:54.786Z" .

FMC:communicatesWith-hasSource
	rdfs:subPropertyOf pig:eligibleSource ;
	rdfs:label "Connects the source of FMC:communicatesWith" ;
	rdfs:domain FMC:communicatesWith ;
	rdfs:range [ owl:unionOf( FMC:Actor uml:Port )] ;
	dcterms:modified "2023-03-15T09:13:54.786Z" .

FMC:communicatesWith-hasTarget
	rdfs:subPropertyOf pig:eligibleTarget ;
	rdfs:label "Connects the target of FMC:communicatesWith" ;
	rdfs:domain FMC:communicatesWith ;
	rdfs:range [ owl:unionOf( FMC:Actor uml:Port )] ;
	dcterms:modified "2023-03-15T09:13:54.786Z" .

FMC:communicatesWith-Shape
	sh:targetClass FMC:communicatesWith ;
	sh:property [ 
		sh:path FMC:communicatesWith-hasSource ;
		sh:class [ owl:unionOf( FMC:Actor uml:Port )] ;
		sh:minCount 1 ;
		sh:maxCount 1
	] ;
	sh:property [ 
		sh:path FMC:communicatesWith-hasTarget ;
		sh:class [ owl:unionOf( FMC:Actor uml:Port )] ;
		sh:minCount 1 ;
		sh:maxCount 1
	] .

SpecIF:contains
	rdfs:subClassOf SpecIF:relates ;
	rdfs:label "contains"@en ;
	rdfs:label "enthält"@de ;
	rdfs:label "contient"@fr ;
	rdfs:comment "General containment, such as:- Package-A *contains* Diagram-B- Collection-1 *contains* DataObject-1.1Not to confound with *[[dcterms:hasPart]]*."@en ;
	dcterms:modified "2024-06-18T12:22:11.959Z" .

SpecIF:contains-hasSource
	rdfs:subPropertyOf pig:eligibleSource ;
	rdfs:label "Connects the source of SpecIF:contains" ;
	rdfs:domain SpecIF:contains ;
	rdfs:range [ owl:unionOf( FMC:Actor FMC:State SpecIF:Collection uml:Package )] ;
	dcterms:modified "2024-06-18T12:22:11.959Z" .

SpecIF:contains-hasTarget
	rdfs:subPropertyOf pig:eligibleTarget ;
	rdfs:label "Connects the target of SpecIF:contains" ;
	rdfs:domain SpecIF:contains ;
	rdfs:range [ owl:unionOf( FMC:Actor FMC:State FMC:Event SpecIF:Collection uml:Package SpecIF:ModelElement pig:View )] ;
	dcterms:modified "2024-06-18T12:22:11.959Z" .

SpecIF:contains-Shape
	sh:targetClass SpecIF:contains ;
	sh:property dcterms:type-Shape ;
	sh:property [ 
		sh:path SpecIF:contains-hasSource ;
		sh:class [ owl:unionOf( FMC:Actor FMC:State SpecIF:Collection uml:Package )] ;
		sh:minCount 1 ;
		sh:maxCount 1
	] ;
	sh:property [ 
		sh:path SpecIF:contains-hasTarget ;
		sh:class [ owl:unionOf( FMC:Actor FMC:State FMC:Event SpecIF:Collection uml:Package SpecIF:ModelElement pig:View )] ;
		sh:minCount 1 ;
		sh:maxCount 1
	] .

SpecIF:isResponsibilityOf
	rdfs:subClassOf pig:Relationship ;
	rdfs:label "is responsibility of" ;
	dcterms:modified "2025-06-24T09:04:26.989Z" .

SpecIF:isResponsibilityOf-hasSource
	rdfs:subPropertyOf pig:eligibleSource ;
	rdfs:label "Connects the source of SpecIF:isResponsibilityOf" ;
	rdfs:domain SpecIF:isResponsibilityOf ;
	dcterms:modified "2025-06-24T09:04:26.989Z" .

SpecIF:isResponsibilityOf-hasTarget
	rdfs:subPropertyOf pig:eligibleTarget ;
	rdfs:label "Connects the target of SpecIF:isResponsibilityOf" ;
	rdfs:domain SpecIF:isResponsibilityOf ;
	dcterms:modified "2025-06-24T09:04:26.989Z" .

SpecIF:isResponsibilityOf-Shape
	sh:targetClass SpecIF:isResponsibilityOf ;
	sh:property [ 
		sh:path SpecIF:isResponsibilityOf-hasSource ;
		sh:minCount 1 ;
		sh:maxCount 1
	] ;
	sh:property [ 
		sh:path SpecIF:isResponsibilityOf-hasTarget ;
		sh:minCount 1 ;
		sh:maxCount 1
	] .

oslc_rm:satisfies
	rdfs:subClassOf pig:Relationship ;
	rdfs:label "satisfies"@en ;
	rdfs:label "erfüllt"@de ;
	rdfs:label "satisfait"@fr ;
	rdfs:comment "<p>The object is satisfied by the subject. <small>(<i>source: <a href=\"http://open-services.net/\">OSLC</a></i>)</small></p><p>SpecIF suggests that the subject is confined to a model element, e.g, a [[FMC:Actor]] or [[FMC:State]], and the object is confined to a [[IREB:Requirement]]. More concretely, an example for this type of statement is 'Component-X <em>satisfies</em> 'Requirement-4711'.</p>"@en ;
	dcterms:modified "2024-06-14T06:49:51.419Z" .

oslc_rm:satisfies-hasSource
	rdfs:subPropertyOf pig:eligibleSource ;
	rdfs:label "Connects the source of oslc_rm:satisfies" ;
	rdfs:domain oslc_rm:satisfies ;
	rdfs:range [ owl:unionOf( FMC:Actor FMC:State FMC:Event SpecIF:Collection DDP:ProductFunction DDP:SystemComponent DDP:ComponentInterface )] ;
	dcterms:modified "2024-06-14T06:49:51.419Z" .

oslc_rm:satisfies-hasTarget
	rdfs:subPropertyOf pig:eligibleTarget ;
	rdfs:label "Connects the target of oslc_rm:satisfies" ;
	rdfs:domain oslc_rm:satisfies ;
	rdfs:range [ owl:unionOf( IREB:Requirement ReqIF-WF:Requirement )] ;
	dcterms:modified "2024-06-14T06:49:51.419Z" .

oslc_rm:satisfies-Shape
	sh:targetClass oslc_rm:satisfies ;
	sh:property [ 
		sh:path oslc_rm:satisfies-hasSource ;
		sh:class [ owl:unionOf( FMC:Actor FMC:State FMC:Event SpecIF:Collection DDP:ProductFunction DDP:SystemComponent DDP:ComponentInterface )] ;
		sh:minCount 1 ;
		sh:maxCount 1
	] ;
	sh:property [ 
		sh:path oslc_rm:satisfies-hasTarget ;
		sh:class [ owl:unionOf( IREB:Requirement ReqIF-WF:Requirement )] ;
		sh:minCount 1 ;
		sh:maxCount 1
	] .

oslc_rm:satisfiedBy
	rdfs:subClassOf pig:Relationship ;
	rdfs:label "satisfied by"@en ;
	rdfs:label "erfüllt von"@de ;
	rdfs:label "satisfait par"@fr ;
	rdfs:comment "<p>The subject is satisfied by the object. For example, a user requirement is satisfied by a system requirement. <small>(<i>source: <a href=\"http://open-services.net/\">OSLC</a></i>)</small></p>" ;
	dcterms:modified "2023-03-08T16:57:09.440Z" .

oslc_rm:satisfiedBy-hasSource
	rdfs:subPropertyOf pig:eligibleSource ;
	rdfs:label "Connects the source of oslc_rm:satisfiedBy" ;
	rdfs:domain oslc_rm:satisfiedBy ;
	rdfs:range [ owl:unionOf( IREB:Requirement ReqIF-WF:Requirement )] ;
	dcterms:modified "2023-03-08T16:57:09.440Z" .

oslc_rm:satisfiedBy-hasTarget
	rdfs:subPropertyOf pig:eligibleTarget ;
	rdfs:label "Connects the target of oslc_rm:satisfiedBy" ;
	rdfs:domain oslc_rm:satisfiedBy ;
	rdfs:range [ owl:unionOf( FMC:Actor FMC:State FMC:Event SpecIF:Collection )] ;
	dcterms:modified "2023-03-08T16:57:09.440Z" .

oslc_rm:satisfiedBy-Shape
	sh:targetClass oslc_rm:satisfiedBy ;
	sh:property [ 
		sh:path oslc_rm:satisfiedBy-hasSource ;
		sh:class [ owl:unionOf( IREB:Requirement ReqIF-WF:Requirement )] ;
		sh:minCount 1 ;
		sh:maxCount 1
	] ;
	sh:property [ 
		sh:path oslc_rm:satisfiedBy-hasTarget ;
		sh:class [ owl:unionOf( FMC:Actor FMC:State FMC:Event SpecIF:Collection )] ;
		sh:minCount 1 ;
		sh:maxCount 1
	] .

SpecIF:serves
	rdfs:subClassOf pig:Relationship ;
	rdfs:label "serves"@en ;
	rdfs:comment "<p>A [[FMC:Actor]] 'serves' a FMC:Actor.</p>"@en ;
	dcterms:modified "2024-07-14T19:43:48.563Z" .

SpecIF:serves-hasSource
	rdfs:subPropertyOf pig:eligibleSource ;
	rdfs:label "Connects the source of SpecIF:serves" ;
	rdfs:domain SpecIF:serves ;
	rdfs:range [ owl:unionOf( FMC:Actor uml:Port )] ;
	dcterms:modified "2024-07-14T19:43:48.563Z" .

SpecIF:serves-hasTarget
	rdfs:subPropertyOf pig:eligibleTarget ;
	rdfs:label "Connects the target of SpecIF:serves" ;
	rdfs:domain SpecIF:serves ;
	rdfs:range [ owl:unionOf( FMC:Actor uml:Port )] ;
	dcterms:modified "2024-07-14T19:43:48.563Z" .

SpecIF:serves-Shape
	sh:targetClass SpecIF:serves ;
	sh:property [ 
		sh:path SpecIF:serves-hasSource ;
		sh:class [ owl:unionOf( FMC:Actor uml:Port )] ;
		sh:minCount 1 ;
		sh:maxCount 1
	] ;
	sh:property [ 
		sh:path SpecIF:serves-hasTarget ;
		sh:class [ owl:unionOf( FMC:Actor uml:Port )] ;
		sh:minCount 1 ;
		sh:maxCount 1
	] .

SpecIF:consumes
	rdfs:subClassOf SpecIF:handles ;
	rdfs:label "consumes"@en ;
	dcterms:modified "2024-07-14T12:45:08.719Z" .

SpecIF:consumes-hasSource
	rdfs:subPropertyOf pig:eligibleSource ;
	rdfs:label "Connects the source of SpecIF:consumes" ;
	rdfs:domain SpecIF:consumes ;
	rdfs:range [ owl:unionOf( FMC:Actor uml:Port SpecIF:ModelElement )] ;
	dcterms:modified "2024-07-14T12:45:08.719Z" .

SpecIF:consumes-hasTarget
	rdfs:subPropertyOf pig:eligibleTarget ;
	rdfs:label "Connects the target of SpecIF:consumes" ;
	rdfs:domain SpecIF:consumes ;
	rdfs:range [ owl:unionOf( FMC:State SpecIF:ModelElement )] ;
	dcterms:modified "2024-07-14T12:45:08.719Z" .

SpecIF:consumes-Shape
	sh:targetClass SpecIF:consumes ;
	sh:property [ 
		sh:path SpecIF:consumes-hasSource ;
		sh:class [ owl:unionOf( FMC:Actor uml:Port SpecIF:ModelElement )] ;
		sh:minCount 1 ;
		sh:maxCount 1
	] ;
	sh:property [ 
		sh:path SpecIF:consumes-hasTarget ;
		sh:class [ owl:unionOf( FMC:State SpecIF:ModelElement )] ;
		sh:minCount 1 ;
		sh:maxCount 1
	] .

SpecIF:provides
	rdfs:subClassOf SpecIF:handles ;
	rdfs:label "provides"@en ;
	dcterms:modified "2024-07-14T12:41:34.601Z" .

SpecIF:provides-hasSource
	rdfs:subPropertyOf pig:eligibleSource ;
	rdfs:label "Connects the source of SpecIF:provides" ;
	rdfs:domain SpecIF:provides ;
	rdfs:range [ owl:unionOf( FMC:Actor uml:Port SpecIF:ModelElement )] ;
	dcterms:modified "2024-07-14T12:41:34.601Z" .

SpecIF:provides-hasTarget
	rdfs:subPropertyOf pig:eligibleTarget ;
	rdfs:label "Connects the target of SpecIF:provides" ;
	rdfs:domain SpecIF:provides ;
	rdfs:range [ owl:unionOf( FMC:State SpecIF:ModelElement )] ;
	dcterms:modified "2024-07-14T12:41:34.601Z" .

SpecIF:provides-Shape
	sh:targetClass SpecIF:provides ;
	sh:property [ 
		sh:path SpecIF:provides-hasSource ;
		sh:class [ owl:unionOf( FMC:Actor uml:Port SpecIF:ModelElement )] ;
		sh:minCount 1 ;
		sh:maxCount 1
	] ;
	sh:property [ 
		sh:path SpecIF:provides-hasTarget ;
		sh:class [ owl:unionOf( FMC:State SpecIF:ModelElement )] ;
		sh:minCount 1 ;
		sh:maxCount 1
	] .

SpecIF:reads
	rdfs:subClassOf SpecIF:accesses ;
	rdfs:label "reads"@en ;
	rdfs:label "liest"@de ;
	rdfs:label "lit"@fr ;
	rdfs:comment "A [[FMC:Actor]] 'reads' a [[FMC:State]]."@en ;
	dcterms:modified "2023-03-15T09:08:53.827Z" .

SpecIF:reads-hasSource
	rdfs:subPropertyOf pig:eligibleSource ;
	rdfs:label "Connects the source of SpecIF:reads" ;
	rdfs:domain SpecIF:reads ;
	rdfs:range [ owl:unionOf( FMC:Actor uml:Port )] ;
	dcterms:modified "2023-03-15T09:08:53.827Z" .

SpecIF:reads-hasTarget
	rdfs:subPropertyOf pig:eligibleTarget ;
	rdfs:label "Connects the target of SpecIF:reads" ;
	rdfs:domain SpecIF:reads ;
	rdfs:range FMC:State ;
	dcterms:modified "2023-03-15T09:08:53.827Z" .

SpecIF:reads-Shape
	sh:targetClass SpecIF:reads ;
	sh:property dcterms:type-Shape ;
	sh:property [ 
		sh:path SpecIF:reads-hasSource ;
		sh:class [ owl:unionOf( FMC:Actor uml:Port )] ;
		sh:minCount 1 ;
		sh:maxCount 1
	] ;
	sh:property [ 
		sh:path SpecIF:reads-hasTarget ;
		sh:class FMC:State ;
		sh:minCount 1 ;
		sh:maxCount 1
	] .

SpecIF:writes
	rdfs:subClassOf SpecIF:accesses ;
	rdfs:label "writes"@en ;
	rdfs:label "schreibt"@de ;
	rdfs:label "écrit"@fr ;
	rdfs:comment "A [[FMC:Actor]] 'writes' (changes) a [[FMC:State]]."@en ;
	dcterms:modified "2023-03-15T09:09:08.696Z" .

SpecIF:writes-hasSource
	rdfs:subPropertyOf pig:eligibleSource ;
	rdfs:label "Connects the source of SpecIF:writes" ;
	rdfs:domain SpecIF:writes ;
	rdfs:range [ owl:unionOf( FMC:Actor uml:Port )] ;
	dcterms:modified "2023-03-15T09:09:08.696Z" .

SpecIF:writes-hasTarget
	rdfs:subPropertyOf pig:eligibleTarget ;
	rdfs:label "Connects the target of SpecIF:writes" ;
	rdfs:domain SpecIF:writes ;
	rdfs:range FMC:State ;
	dcterms:modified "2023-03-15T09:09:08.696Z" .

SpecIF:writes-Shape
	sh:targetClass SpecIF:writes ;
	sh:property dcterms:type-Shape ;
	sh:property [ 
		sh:path SpecIF:writes-hasSource ;
		sh:class [ owl:unionOf( FMC:Actor uml:Port )] ;
		sh:minCount 1 ;
		sh:maxCount 1
	] ;
	sh:property [ 
		sh:path SpecIF:writes-hasTarget ;
		sh:class FMC:State ;
		sh:minCount 1 ;
		sh:maxCount 1
	] .

SpecIF:realizedBy
	rdfs:subClassOf pig:Relationship ;
	rdfs:label "is realized by"@en ;
	rdfs:label "wird realisiert von"@de ;
	rdfs:comment "A business capability is realized by a business function or a business function is realized by an application component."@en ;
	dcterms:modified "2025-01-16T02:42:49.356Z" .

SpecIF:realizedBy-hasSource
	rdfs:subPropertyOf pig:eligibleSource ;
	rdfs:label "Connects the source of SpecIF:realizedBy" ;
	rdfs:domain SpecIF:realizedBy ;
	dcterms:modified "2025-01-16T02:42:49.356Z" .

SpecIF:realizedBy-hasTarget
	rdfs:subPropertyOf pig:eligibleTarget ;
	rdfs:label "Connects the target of SpecIF:realizedBy" ;
	rdfs:domain SpecIF:realizedBy ;
	dcterms:modified "2025-01-16T02:42:49.356Z" .

SpecIF:realizedBy-Shape
	sh:targetClass SpecIF:realizedBy ;
	sh:property [ 
		sh:path SpecIF:realizedBy-hasSource ;
		sh:minCount 1 ;
		sh:maxCount 1
	] ;
	sh:property [ 
		sh:path SpecIF:realizedBy-hasTarget ;
		sh:minCount 1 ;
		sh:maxCount 1
	] .

ArchiMate:Realization
	rdfs:subClassOf ArchiMate:Uniting ;
	rdfs:label "realizes"@en ;
	rdfs:comment "A business function realizes a business capability or an application component realizes a business function."@en ;
	dcterms:modified "2025-06-17T07:47:48.669Z" .

ArchiMate:Realization-hasSource
	rdfs:subPropertyOf pig:eligibleSource ;
	rdfs:label "Connects the source of ArchiMate:Realization" ;
	rdfs:domain ArchiMate:Realization ;
	dcterms:modified "2025-06-17T07:47:48.669Z" .

ArchiMate:Realization-hasTarget
	rdfs:subPropertyOf pig:eligibleTarget ;
	rdfs:label "Connects the target of ArchiMate:Realization" ;
	rdfs:domain ArchiMate:Realization ;
	dcterms:modified "2025-06-17T07:47:48.669Z" .

ArchiMate:Realization-Shape
	sh:targetClass ArchiMate:Realization ;
	sh:property dcterms:type-Shape ;
	sh:property [ 
		sh:path ArchiMate:Realization-hasSource ;
		sh:minCount 1 ;
		sh:maxCount 1
	] ;
	sh:property [ 
		sh:path ArchiMate:Realization-hasTarget ;
		sh:minCount 1 ;
		sh:maxCount 1
	] .

ArchiMate:Assignment
	rdfs:subClassOf ArchiMate:Uniting ;
	rdfs:label "is assigned to"@en ;
	rdfs:comment "<p>The assignment relationship represents the allocation of responsibility, performance of behavior, storage, or execution.</p>"@en ;
	dcterms:modified "2025-08-05T16:52:47.745Z" .

ArchiMate:Assignment-hasSource
	rdfs:subPropertyOf pig:eligibleSource ;
	rdfs:label "Connects the source of ArchiMate:Assignment" ;
	rdfs:domain ArchiMate:Assignment ;
	dcterms:modified "2025-08-05T16:52:47.745Z" .

ArchiMate:Assignment-hasTarget
	rdfs:subPropertyOf pig:eligibleTarget ;
	rdfs:label "Connects the target of ArchiMate:Assignment" ;
	rdfs:domain ArchiMate:Assignment ;
	dcterms:modified "2025-08-05T16:52:47.745Z" .

ArchiMate:Assignment-Shape
	sh:targetClass ArchiMate:Assignment ;
	sh:property dcterms:type-Shape ;
	sh:property [ 
		sh:path ArchiMate:Assignment-hasSource ;
		sh:minCount 1 ;
		sh:maxCount 1
	] ;
	sh:property [ 
		sh:path ArchiMate:Assignment-hasTarget ;
		sh:minCount 1 ;
		sh:maxCount 1
	] .

FMC:sendsTo
	rdfs:subClassOf FMC:communicatesWith ;
	rdfs:label "sends to"@en ;
	rdfs:label "sendet an"@de ;
	rdfs:label "envoie à"@fr ;
	rdfs:comment "A [[FMC:Actor]] 'sends' a message to a [[FMC:Actor]]."@en ;
	dcterms:modified "2023-03-15T09:14:09.263Z" .

FMC:sendsTo-hasSource
	rdfs:subPropertyOf pig:eligibleSource ;
	rdfs:label "Connects the source of FMC:sendsTo" ;
	rdfs:domain FMC:sendsTo ;
	rdfs:range FMC:Actor ;
	dcterms:modified "2023-03-15T09:14:09.263Z" .

FMC:sendsTo-hasTarget
	rdfs:subPropertyOf pig:eligibleTarget ;
	rdfs:label "Connects the target of FMC:sendsTo" ;
	rdfs:domain FMC:sendsTo ;
	rdfs:range FMC:Actor ;
	dcterms:modified "2023-03-15T09:14:09.263Z" .

FMC:sendsTo-Shape
	sh:targetClass FMC:sendsTo ;
	sh:property [ 
		sh:path FMC:sendsTo-hasSource ;
		sh:class FMC:Actor ;
		sh:minCount 1 ;
		sh:maxCount 1
	] ;
	sh:property [ 
		sh:path FMC:sendsTo-hasTarget ;
		sh:class FMC:Actor ;
		sh:minCount 1 ;
		sh:maxCount 1
	] .

FMC:receivesFrom
	rdfs:subClassOf FMC:communicatesWith ;
	rdfs:label "receives from"@en ;
	rdfs:label "empfängt von"@de ;
	rdfs:label "reçoit de"@fr ;
	rdfs:comment "A [[FMC:Actor]] 'receives' a message from a [[FMC:Actor]]."@en ;
	dcterms:modified "2023-03-15T09:14:22.685Z" .

FMC:receivesFrom-hasSource
	rdfs:subPropertyOf pig:eligibleSource ;
	rdfs:label "Connects the source of FMC:receivesFrom" ;
	rdfs:domain FMC:receivesFrom ;
	rdfs:range FMC:Actor ;
	dcterms:modified "2023-03-15T09:14:22.685Z" .

FMC:receivesFrom-hasTarget
	rdfs:subPropertyOf pig:eligibleTarget ;
	rdfs:label "Connects the target of FMC:receivesFrom" ;
	rdfs:domain FMC:receivesFrom ;
	rdfs:range FMC:Actor ;
	dcterms:modified "2023-03-15T09:14:22.685Z" .

FMC:receivesFrom-Shape
	sh:targetClass FMC:receivesFrom ;
	sh:property [ 
		sh:path FMC:receivesFrom-hasSource ;
		sh:class FMC:Actor ;
		sh:minCount 1 ;
		sh:maxCount 1
	] ;
	sh:property [ 
		sh:path FMC:receivesFrom-hasTarget ;
		sh:class FMC:Actor ;
		sh:minCount 1 ;
		sh:maxCount 1
	] .

SpecIF:follows
	rdfs:subClassOf pig:Relationship ;
	rdfs:label "follows"@en ;
	rdfs:label "folgt auf"@de ;
	rdfs:label "succèdes à"@fr ;
	rdfs:comment "A [[FMC:Actor]] 'follows' a [[FMC:Actor]]; e.g. in a business process or activity flow."@en ;
	dcterms:modified "2023-07-16T13:09:55.680Z" .

SpecIF:follows-hasSource
	rdfs:subPropertyOf pig:eligibleSource ;
	rdfs:label "Connects the source of SpecIF:follows" ;
	rdfs:domain SpecIF:follows ;
	rdfs:range FMC:Actor ;
	dcterms:modified "2023-07-16T13:09:55.680Z" .

SpecIF:follows-hasTarget
	rdfs:subPropertyOf pig:eligibleTarget ;
	rdfs:label "Connects the target of SpecIF:follows" ;
	rdfs:domain SpecIF:follows ;
	rdfs:range FMC:Actor ;
	dcterms:modified "2023-07-16T13:09:55.680Z" .

SpecIF:follows-Shape
	sh:targetClass SpecIF:follows ;
	sh:property [ 
		sh:path SpecIF:follows-hasSource ;
		sh:class FMC:Actor ;
		sh:minCount 1 ;
		sh:maxCount 1
	] ;
	sh:property [ 
		sh:path SpecIF:follows-hasTarget ;
		sh:class FMC:Actor ;
		sh:minCount 1 ;
		sh:maxCount 1
	] .

SpecIF:precedes
	rdfs:subClassOf pig:Relationship ;
	rdfs:label "precedes"@en ;
	rdfs:label "ist Vorgänger von"@de ;
	rdfs:label "précède"@fr ;
	rdfs:comment "A [[FMC:Actor]] 'precedes' a [[FMC:Actor]]; e.g. in a business process or activity flow."@en ;
	dcterms:modified "2023-07-16T13:14:41.553Z" .

SpecIF:precedes-hasSource
	rdfs:subPropertyOf pig:eligibleSource ;
	rdfs:label "Connects the source of SpecIF:precedes" ;
	rdfs:domain SpecIF:precedes ;
	rdfs:range FMC:Actor ;
	dcterms:modified "2023-07-16T13:14:41.553Z" .

SpecIF:precedes-hasTarget
	rdfs:subPropertyOf pig:eligibleTarget ;
	rdfs:label "Connects the target of SpecIF:precedes" ;
	rdfs:domain SpecIF:precedes ;
	rdfs:range FMC:Actor ;
	dcterms:modified "2023-07-16T13:14:41.553Z" .

SpecIF:precedes-Shape
	sh:targetClass SpecIF:precedes ;
	sh:property [ 
		sh:path SpecIF:precedes-hasSource ;
		sh:class FMC:Actor ;
		sh:minCount 1 ;
		sh:maxCount 1
	] ;
	sh:property [ 
		sh:path SpecIF:precedes-hasTarget ;
		sh:class FMC:Actor ;
		sh:minCount 1 ;
		sh:maxCount 1
	] .

SpecIF:dependsOn
	rdfs:subClassOf pig:Relationship ;
	rdfs:label "depends on"@en ;
	rdfs:label "hängt ab von"@de ;
	rdfs:label "depend de"@fr ;
	rdfs:comment "<p>A [[IREB:Requirement]] 'depends on' another [[IREB:Requirement]].</p>"@en ;
	dcterms:modified "2023-07-16T13:15:43.014Z" .

SpecIF:dependsOn-hasSource
	rdfs:subPropertyOf pig:eligibleSource ;
	rdfs:label "Connects the source of SpecIF:dependsOn" ;
	rdfs:domain SpecIF:dependsOn ;
	rdfs:range [ owl:unionOf( IREB:Requirement ReqIF-WF:Requirement )] ;
	dcterms:modified "2023-07-16T13:15:43.014Z" .

SpecIF:dependsOn-hasTarget
	rdfs:subPropertyOf pig:eligibleTarget ;
	rdfs:label "Connects the target of SpecIF:dependsOn" ;
	rdfs:domain SpecIF:dependsOn ;
	rdfs:range [ owl:unionOf( IREB:Requirement ReqIF-WF:Requirement )] ;
	dcterms:modified "2023-07-16T13:15:43.014Z" .

SpecIF:dependsOn-Shape
	sh:targetClass SpecIF:dependsOn ;
	sh:property [ 
		sh:path SpecIF:dependsOn-hasSource ;
		sh:class [ owl:unionOf( IREB:Requirement ReqIF-WF:Requirement )] ;
		sh:minCount 1 ;
		sh:maxCount 1
	] ;
	sh:property [ 
		sh:path SpecIF:dependsOn-hasTarget ;
		sh:class [ owl:unionOf( IREB:Requirement ReqIF-WF:Requirement )] ;
		sh:minCount 1 ;
		sh:maxCount 1
	] .

sysml:Usage
	rdfs:subClassOf pig:Relationship ;
	rdfs:label "uses"@en ;
	rdfs:label "benutzt"@de ;
	rdfs:label "utilise"@fr ;
	dcterms:modified "2024-06-18T06:47:42.028Z" .

sysml:Usage-hasSource
	rdfs:subPropertyOf pig:eligibleSource ;
	rdfs:label "Connects the source of sysml:Usage" ;
	rdfs:domain sysml:Usage ;
	dcterms:modified "2024-06-18T06:47:42.028Z" .

sysml:Usage-hasTarget
	rdfs:subPropertyOf pig:eligibleTarget ;
	rdfs:label "Connects the target of sysml:Usage" ;
	rdfs:domain sysml:Usage ;
	dcterms:modified "2024-06-18T06:47:42.028Z" .

sysml:Usage-Shape
	sh:targetClass sysml:Usage ;
	sh:property [ 
		sh:path sysml:Usage-hasSource ;
		sh:minCount 1 ;
		sh:maxCount 1
	] ;
	sh:property [ 
		sh:path sysml:Usage-hasTarget ;
		sh:minCount 1 ;
		sh:maxCount 1
	] .

sysml:Derive
	rdfs:subClassOf pig:Relationship ;
	rdfs:label "derived from"@en ;
	rdfs:label "abgeleitet von"@de ;
	rdfs:label "dérivé de"@fr ;
	rdfs:comment "<p>A [[IREB:Requirement]] 'is derived from' another [[IREB:Requirement]].</p>"@en ;
	dcterms:modified "2024-06-18T07:00:44.641Z" .

sysml:Derive-hasSource
	rdfs:subPropertyOf pig:eligibleSource ;
	rdfs:label "Connects the source of sysml:Derive" ;
	rdfs:domain sysml:Derive ;
	rdfs:range [ owl:unionOf( IREB:Requirement ReqIF-WF:Requirement )] ;
	dcterms:modified "2024-06-18T07:00:44.641Z" .

sysml:Derive-hasTarget
	rdfs:subPropertyOf pig:eligibleTarget ;
	rdfs:label "Connects the target of sysml:Derive" ;
	rdfs:domain sysml:Derive ;
	rdfs:range [ owl:unionOf( IREB:Requirement ReqIF-WF:Requirement )] ;
	dcterms:modified "2024-06-18T07:00:44.641Z" .

sysml:Derive-Shape
	sh:targetClass sysml:Derive ;
	sh:property [ 
		sh:path sysml:Derive-hasSource ;
		sh:class [ owl:unionOf( IREB:Requirement ReqIF-WF:Requirement )] ;
		sh:minCount 1 ;
		sh:maxCount 1
	] ;
	sh:property [ 
		sh:path sysml:Derive-hasTarget ;
		sh:class [ owl:unionOf( IREB:Requirement ReqIF-WF:Requirement )] ;
		sh:minCount 1 ;
		sh:maxCount 1
	] .

sysml:Allocate
	rdfs:subClassOf pig:Relationship ;
	rdfs:label "is allocated to"@en ;
	rdfs:label "zugeordnet zu"@de ;
	rdfs:label "allouée à"@fr ;
	rdfs:comment "<p>An [[FMC:Actor]] is allocated to another [[FMC:Actor]] (e.g. a logical function is allocated to a physical component.</p>"@en ;
	dcterms:modified "2025-09-06T14:59:03.739Z" .

sysml:Allocate-hasSource
	rdfs:subPropertyOf pig:eligibleSource ;
	rdfs:label "Connects the source of sysml:Allocate" ;
	rdfs:domain sysml:Allocate ;
	rdfs:range SpecIF:ModelElement ;
	dcterms:modified "2025-09-06T14:59:03.739Z" .

sysml:Allocate-hasTarget
	rdfs:subPropertyOf pig:eligibleTarget ;
	rdfs:label "Connects the target of sysml:Allocate" ;
	rdfs:domain sysml:Allocate ;
	rdfs:range SpecIF:ModelElement ;
	dcterms:modified "2025-09-06T14:59:03.739Z" .

sysml:Allocate-Shape
	sh:targetClass sysml:Allocate ;
	sh:property [ 
		sh:path sysml:Allocate-hasSource ;
		sh:class SpecIF:ModelElement ;
		sh:minCount 1 ;
		sh:maxCount 1
	] ;
	sh:property [ 
		sh:path sysml:Allocate-hasTarget ;
		sh:class SpecIF:ModelElement ;
		sh:minCount 1 ;
		sh:maxCount 1
	] .

IREB:refines
	rdfs:subClassOf pig:Relationship ;
	rdfs:label "refines"@en ;
	rdfs:label "verfeinert"@de ;
	rdfs:label "affine"@fr ;
	rdfs:comment "<p>A [[IREB:Requirement]] 'refines' another [[IREB:Requirement]].</p>"@en ;
	dcterms:modified "2023-08-08T21:08:32.367Z" .

IREB:refines-hasSource
	rdfs:subPropertyOf pig:eligibleSource ;
	rdfs:label "Connects the source of IREB:refines" ;
	rdfs:domain IREB:refines ;
	rdfs:range [ owl:unionOf( IREB:Requirement ReqIF-WF:Requirement )] ;
	dcterms:modified "2023-08-08T21:08:32.367Z" .

IREB:refines-hasTarget
	rdfs:subPropertyOf pig:eligibleTarget ;
	rdfs:label "Connects the target of IREB:refines" ;
	rdfs:domain IREB:refines ;
	rdfs:range [ owl:unionOf( IREB:Requirement ReqIF-WF:Requirement )] ;
	dcterms:modified "2023-08-08T21:08:32.367Z" .

IREB:refines-Shape
	sh:targetClass IREB:refines ;
	sh:property [ 
		sh:path IREB:refines-hasSource ;
		sh:class [ owl:unionOf( IREB:Requirement ReqIF-WF:Requirement )] ;
		sh:minCount 1 ;
		sh:maxCount 1
	] ;
	sh:property [ 
		sh:path IREB:refines-hasTarget ;
		sh:class [ owl:unionOf( IREB:Requirement ReqIF-WF:Requirement )] ;
		sh:minCount 1 ;
		sh:maxCount 1
	] .

IREB:refinedBy
	rdfs:subClassOf pig:Relationship ;
	rdfs:label "refined by"@en ;
	rdfs:label "verfeinert durch"@de ;
	rdfs:label "affiné de"@fr ;
	rdfs:comment "<p>A [[IREB:Requirement]] 'is refined by' another [[IREB:Requirement]].</p>"@en ;
	dcterms:modified "2025-09-05T12:30:00.059Z" .

IREB:refinedBy-hasSource
	rdfs:subPropertyOf pig:eligibleSource ;
	rdfs:label "Connects the source of IREB:refinedBy" ;
	rdfs:domain IREB:refinedBy ;
	dcterms:modified "2025-09-05T12:30:00.059Z" .

IREB:refinedBy-hasTarget
	rdfs:subPropertyOf pig:eligibleTarget ;
	rdfs:label "Connects the target of IREB:refinedBy" ;
	rdfs:domain IREB:refinedBy ;
	dcterms:modified "2025-09-05T12:30:00.059Z" .

IREB:refinedBy-Shape
	sh:targetClass IREB:refinedBy ;
	sh:property [ 
		sh:path IREB:refinedBy-hasSource ;
		sh:minCount 1 ;
		sh:maxCount 1
	] ;
	sh:property [ 
		sh:path IREB:refinedBy-hasTarget ;
		sh:minCount 1 ;
		sh:maxCount 1
	] .

SpecIF:duplicates
	rdfs:subClassOf pig:Relationship ;
	rdfs:label "duplicates"@en ;
	rdfs:label "dupliziert"@de ;
	rdfs:label "reprend"@fr ;
	rdfs:comment "<p>A [[IREB:Requirement]] 'duplicates' another [[IREB:Requirement]].</p>"@en ;
	dcterms:modified "2023-07-16T15:01:40.623Z" .

SpecIF:duplicates-hasSource
	rdfs:subPropertyOf pig:eligibleSource ;
	rdfs:label "Connects the source of SpecIF:duplicates" ;
	rdfs:domain SpecIF:duplicates ;
	rdfs:range [ owl:unionOf( IREB:Requirement ReqIF-WF:Requirement )] ;
	dcterms:modified "2023-07-16T15:01:40.623Z" .

SpecIF:duplicates-hasTarget
	rdfs:subPropertyOf pig:eligibleTarget ;
	rdfs:label "Connects the target of SpecIF:duplicates" ;
	rdfs:domain SpecIF:duplicates ;
	rdfs:range [ owl:unionOf( IREB:Requirement ReqIF-WF:Requirement )] ;
	dcterms:modified "2023-07-16T15:01:40.623Z" .

SpecIF:duplicates-Shape
	sh:targetClass SpecIF:duplicates ;
	sh:property [ 
		sh:path SpecIF:duplicates-hasSource ;
		sh:class [ owl:unionOf( IREB:Requirement ReqIF-WF:Requirement )] ;
		sh:minCount 1 ;
		sh:maxCount 1
	] ;
	sh:property [ 
		sh:path SpecIF:duplicates-hasTarget ;
		sh:class [ owl:unionOf( IREB:Requirement ReqIF-WF:Requirement )] ;
		sh:minCount 1 ;
		sh:maxCount 1
	] .

dcterms:replaces
	rdfs:subClassOf pig:Relationship ;
	rdfs:label "replaces"@en ;
	rdfs:label "ersetzt"@de ;
	rdfs:label "remplaces"@fr ;
	rdfs:comment "<p>A [[IREB:Requirement]] 'replaces' another [[IREB:Requirement]].</p>"@en ;
	dcterms:modified "2024-02-12T16:07:03.611Z" .

dcterms:replaces-hasSource
	rdfs:subPropertyOf pig:eligibleSource ;
	rdfs:label "Connects the source of dcterms:replaces" ;
	rdfs:domain dcterms:replaces ;
	rdfs:range [ owl:unionOf( IREB:Requirement ReqIF-WF:Requirement )] ;
	dcterms:modified "2024-02-12T16:07:03.611Z" .

dcterms:replaces-hasTarget
	rdfs:subPropertyOf pig:eligibleTarget ;
	rdfs:label "Connects the target of dcterms:replaces" ;
	rdfs:domain dcterms:replaces ;
	rdfs:range [ owl:unionOf( IREB:Requirement ReqIF-WF:Requirement )] ;
	dcterms:modified "2024-02-12T16:07:03.611Z" .

dcterms:replaces-Shape
	sh:targetClass dcterms:replaces ;
	sh:property rdfs:comment-Shape ;
	sh:property [ 
		sh:path dcterms:replaces-hasSource ;
		sh:class [ owl:unionOf( IREB:Requirement ReqIF-WF:Requirement )] ;
		sh:minCount 1 ;
		sh:maxCount 1
	] ;
	sh:property [ 
		sh:path dcterms:replaces-hasTarget ;
		sh:class [ owl:unionOf( IREB:Requirement ReqIF-WF:Requirement )] ;
		sh:minCount 1 ;
		sh:maxCount 1
	] .

SpecIF:contradicts
	rdfs:subClassOf pig:Relationship ;
	rdfs:label "contradicts"@en ;
	rdfs:label "widerspricht"@de ;
	rdfs:label "contredit"@fr ;
	rdfs:comment "<p>A [[IREB:Requirement]] 'contradicts' another [[IREB:Requirement]].</p>"@en ;
	dcterms:modified "2023-07-16T15:02:23.500Z" .

SpecIF:contradicts-hasSource
	rdfs:subPropertyOf pig:eligibleSource ;
	rdfs:label "Connects the source of SpecIF:contradicts" ;
	rdfs:domain SpecIF:contradicts ;
	rdfs:range [ owl:unionOf( IREB:Requirement ReqIF-WF:Requirement )] ;
	dcterms:modified "2023-07-16T15:02:23.500Z" .

SpecIF:contradicts-hasTarget
	rdfs:subPropertyOf pig:eligibleTarget ;
	rdfs:label "Connects the target of SpecIF:contradicts" ;
	rdfs:domain SpecIF:contradicts ;
	rdfs:range [ owl:unionOf( IREB:Requirement ReqIF-WF:Requirement )] ;
	dcterms:modified "2023-07-16T15:02:23.500Z" .

SpecIF:contradicts-Shape
	sh:targetClass SpecIF:contradicts ;
	sh:property [ 
		sh:path SpecIF:contradicts-hasSource ;
		sh:class [ owl:unionOf( IREB:Requirement ReqIF-WF:Requirement )] ;
		sh:minCount 1 ;
		sh:maxCount 1
	] ;
	sh:property [ 
		sh:path SpecIF:contradicts-hasTarget ;
		sh:class [ owl:unionOf( IREB:Requirement ReqIF-WF:Requirement )] ;
		sh:minCount 1 ;
		sh:maxCount 1
	] .

SpecIF:isAssociatedWith
	rdfs:subClassOf SpecIF:relates ;
	rdfs:label "associated with"@en ;
	rdfs:label "assoziiert mit"@de ;
	rdfs:label "associé avec"@fr ;
	rdfs:comment "<p>A [[FMC:State]] is associated with another [[FMC:State]] (e.g. a class is associated with another class, as shown in a UML Class Diagram).</p>"@en ;
	dcterms:modified "2024-07-17T14:56:18.430Z" .

SpecIF:isAssociatedWith-hasSource
	rdfs:subPropertyOf pig:eligibleSource ;
	rdfs:label "Connects the source of SpecIF:isAssociatedWith" ;
	rdfs:domain SpecIF:isAssociatedWith ;
	dcterms:modified "2024-07-17T14:56:18.430Z" .

SpecIF:isAssociatedWith-hasTarget
	rdfs:subPropertyOf pig:eligibleTarget ;
	rdfs:label "Connects the target of SpecIF:isAssociatedWith" ;
	rdfs:domain SpecIF:isAssociatedWith ;
	dcterms:modified "2024-07-17T14:56:18.430Z" .

SpecIF:isAssociatedWith-Shape
	sh:targetClass SpecIF:isAssociatedWith ;
	sh:property dcterms:type-Shape ;
	sh:property [ 
		sh:path SpecIF:isAssociatedWith-hasSource ;
		sh:minCount 1 ;
		sh:maxCount 1
	] ;
	sh:property [ 
		sh:path SpecIF:isAssociatedWith-hasTarget ;
		sh:minCount 1 ;
		sh:maxCount 1
	] .

uml:Aggregation
	rdfs:subClassOf SpecIF:relates ;
	rdfs:label "aggregates"@en ;
	rdfs:label "aggregiert"@de ;
	rdfs:label "agrégat"@fr ;
	rdfs:comment "<p>An [[FMC:Actor]] aggregates another [[FMC:Actor]].</p><p>If amounts or things are aggregated, they are added together and considered as a single amount or thing.<i><small>Source: <a href=\"https://www.collinsdictionary.com/dictionary/english/aggregate\">Collins Dictionary</a></small></i></p>"@en ;
	dcterms:modified "2025-09-06T14:55:24.185Z" .

uml:Aggregation-hasSource
	rdfs:subPropertyOf pig:eligibleSource ;
	rdfs:label "Connects the source of uml:Aggregation" ;
	rdfs:domain uml:Aggregation ;
	dcterms:modified "2025-09-06T14:55:24.185Z" .

uml:Aggregation-hasTarget
	rdfs:subPropertyOf pig:eligibleTarget ;
	rdfs:label "Connects the target of uml:Aggregation" ;
	rdfs:domain uml:Aggregation ;
	dcterms:modified "2025-09-06T14:55:24.185Z" .

uml:Aggregation-Shape
	sh:targetClass uml:Aggregation ;
	sh:property dcterms:type-Shape ;
	sh:property [ 
		sh:path uml:Aggregation-hasSource ;
		sh:minCount 1 ;
		sh:maxCount 1
	] ;
	sh:property [ 
		sh:path uml:Aggregation-hasTarget ;
		sh:minCount 1 ;
		sh:maxCount 1
	] .

uml:extends
	rdfs:subClassOf pig:Relationship ;
	rdfs:label "extends"@en ;
	rdfs:label "erweitert"@de ;
	rdfs:label "s'étend"@fr ;
	rdfs:comment "<p>An [[FMC:Actor]] «UseCase» extends another [[FMC:Actor]] «UseCase».</p>"@en ;
	dcterms:modified "2023-07-16T15:23:43.133Z" .

uml:extends-hasSource
	rdfs:subPropertyOf pig:eligibleSource ;
	rdfs:label "Connects the source of uml:extends" ;
	rdfs:domain uml:extends ;
	rdfs:range FMC:Actor ;
	dcterms:modified "2023-07-16T15:23:43.133Z" .

uml:extends-hasTarget
	rdfs:subPropertyOf pig:eligibleTarget ;
	rdfs:label "Connects the target of uml:extends" ;
	rdfs:domain uml:extends ;
	rdfs:range FMC:Actor ;
	dcterms:modified "2023-07-16T15:23:43.133Z" .

uml:extends-Shape
	sh:targetClass uml:extends ;
	sh:property [ 
		sh:path uml:extends-hasSource ;
		sh:class FMC:Actor ;
		sh:minCount 1 ;
		sh:maxCount 1
	] ;
	sh:property [ 
		sh:path uml:extends-hasTarget ;
		sh:class FMC:Actor ;
		sh:minCount 1 ;
		sh:maxCount 1
	] .

sysml:includes
	rdfs:subClassOf pig:Relationship ;
	rdfs:label "includes"@en ;
	rdfs:label "inkludiert"@de ;
	rdfs:label "inclut"@fr ;
	rdfs:comment "<p>An [[FMC:Actor]] «UseCase» includes another [[FMC:Actor]] «UseCase».</p>"@en ;
	dcterms:modified "2023-07-16T15:20:39.094Z" .

sysml:includes-hasSource
	rdfs:subPropertyOf pig:eligibleSource ;
	rdfs:label "Connects the source of sysml:includes" ;
	rdfs:domain sysml:includes ;
	rdfs:range FMC:Actor ;
	dcterms:modified "2023-07-16T15:20:39.094Z" .

sysml:includes-hasTarget
	rdfs:subPropertyOf pig:eligibleTarget ;
	rdfs:label "Connects the target of sysml:includes" ;
	rdfs:domain sysml:includes ;
	rdfs:range FMC:Actor ;
	dcterms:modified "2023-07-16T15:20:39.094Z" .

sysml:includes-Shape
	sh:targetClass sysml:includes ;
	sh:property [ 
		sh:path sysml:includes-hasSource ;
		sh:class FMC:Actor ;
		sh:minCount 1 ;
		sh:maxCount 1
	] ;
	sh:property [ 
		sh:path sysml:includes-hasTarget ;
		sh:class FMC:Actor ;
		sh:minCount 1 ;
		sh:maxCount 1
	] .

uml:Realization
	rdfs:subClassOf pig:Relationship ;
	rdfs:label "realizes"@en ;
	rdfs:label "realisiert"@de ;
	rdfs:label "réalise"@fr ;
	rdfs:comment "A component *realizes' a function."@en ;
	dcterms:modified "2024-06-19T23:49:22.932Z" .

uml:Realization-hasSource
	rdfs:subPropertyOf pig:eligibleSource ;
	rdfs:label "Connects the source of uml:Realization" ;
	rdfs:domain uml:Realization ;
	dcterms:modified "2024-06-19T23:49:22.932Z" .

uml:Realization-hasTarget
	rdfs:subPropertyOf pig:eligibleTarget ;
	rdfs:label "Connects the target of uml:Realization" ;
	rdfs:domain uml:Realization ;
	dcterms:modified "2024-06-19T23:49:22.932Z" .

uml:Realization-Shape
	sh:targetClass uml:Realization ;
	sh:property [ 
		sh:path uml:Realization-hasSource ;
		sh:minCount 1 ;
		sh:maxCount 1
	] ;
	sh:property [ 
		sh:path uml:Realization-hasTarget ;
		sh:minCount 1 ;
		sh:maxCount 1
	] .

uml:ownedBehavior
	rdfs:subClassOf pig:Relationship ;
	rdfs:label "has Behavior" ;
	dcterms:modified "2025-04-21T17:40:00.590Z" .

uml:ownedBehavior-hasSource
	rdfs:subPropertyOf pig:eligibleSource ;
	rdfs:label "Connects the source of uml:ownedBehavior" ;
	rdfs:domain uml:ownedBehavior ;
	dcterms:modified "2025-04-21T17:40:00.590Z" .

uml:ownedBehavior-hasTarget
	rdfs:subPropertyOf pig:eligibleTarget ;
	rdfs:label "Connects the target of uml:ownedBehavior" ;
	rdfs:domain uml:ownedBehavior ;
	rdfs:range [ owl:unionOf( uml:StateMachine uml:Activity FMC:Actor uml:UseCase )] ;
	dcterms:modified "2025-04-21T17:40:00.590Z" .

uml:ownedBehavior-Shape
	sh:targetClass uml:ownedBehavior ;
	sh:property [ 
		sh:path uml:ownedBehavior-hasSource ;
		sh:minCount 1 ;
		sh:maxCount 1
	] ;
	sh:property [ 
		sh:path uml:ownedBehavior-hasTarget ;
		sh:class [ owl:unionOf( uml:StateMachine uml:Activity FMC:Actor uml:UseCase )] ;
		sh:minCount 1 ;
		sh:maxCount 1
	] .

uml:Trigger
	rdfs:subClassOf pig:Relationship ;
	rdfs:label "triggers" ;
	dcterms:modified "2025-04-22T09:22:53.072Z" .

uml:Trigger-hasSource
	rdfs:subPropertyOf pig:eligibleSource ;
	rdfs:label "Connects the source of uml:Trigger" ;
	rdfs:domain uml:Trigger ;
	dcterms:modified "2025-04-22T09:22:53.072Z" .

uml:Trigger-hasTarget
	rdfs:subPropertyOf pig:eligibleTarget ;
	rdfs:label "Connects the target of uml:Trigger" ;
	rdfs:domain uml:Trigger ;
	dcterms:modified "2025-04-22T09:22:53.072Z" .

uml:Trigger-Shape
	sh:targetClass uml:Trigger ;
	sh:property [ 
		sh:path uml:Trigger-hasSource ;
		sh:minCount 1 ;
		sh:maxCount 1
	] ;
	sh:property [ 
		sh:path uml:Trigger-hasTarget ;
		sh:minCount 1 ;
		sh:maxCount 1
	] .

uml:TransitionSource
	rdfs:subClassOf pig:Relationship ;
	rdfs:label "starts from" ;
	dcterms:modified "2025-04-22T13:49:51.249Z" .

uml:TransitionSource-hasSource
	rdfs:subPropertyOf pig:eligibleSource ;
	rdfs:label "Connects the source of uml:TransitionSource" ;
	rdfs:domain uml:TransitionSource ;
	rdfs:range [ owl:unionOf( uml:Transition FMC:Actor )] ;
	dcterms:modified "2025-04-22T13:49:51.249Z" .

uml:TransitionSource-hasTarget
	rdfs:subPropertyOf pig:eligibleTarget ;
	rdfs:label "Connects the target of uml:TransitionSource" ;
	rdfs:domain uml:TransitionSource ;
	rdfs:range [ owl:unionOf( uml:State FMC:State )] ;
	dcterms:modified "2025-04-22T13:49:51.249Z" .

uml:TransitionSource-Shape
	sh:targetClass uml:TransitionSource ;
	sh:property [ 
		sh:path uml:TransitionSource-hasSource ;
		sh:class [ owl:unionOf( uml:Transition FMC:Actor )] ;
		sh:minCount 1 ;
		sh:maxCount 1
	] ;
	sh:property [ 
		sh:path uml:TransitionSource-hasTarget ;
		sh:class [ owl:unionOf( uml:State FMC:State )] ;
		sh:minCount 1 ;
		sh:maxCount 1
	] .

uml:TransitionTarget
	rdfs:subClassOf pig:Relationship ;
	rdfs:label "ends at" ;
	dcterms:modified "2025-04-22T13:50:34.458Z" .

uml:TransitionTarget-hasSource
	rdfs:subPropertyOf pig:eligibleSource ;
	rdfs:label "Connects the source of uml:TransitionTarget" ;
	rdfs:domain uml:TransitionTarget ;
	rdfs:range [ owl:unionOf( uml:Transition FMC:Actor )] ;
	dcterms:modified "2025-04-22T13:50:34.458Z" .

uml:TransitionTarget-hasTarget
	rdfs:subPropertyOf pig:eligibleTarget ;
	rdfs:label "Connects the target of uml:TransitionTarget" ;
	rdfs:domain uml:TransitionTarget ;
	rdfs:range [ owl:unionOf( uml:State FMC:State )] ;
	dcterms:modified "2025-04-22T13:50:34.458Z" .

uml:TransitionTarget-Shape
	sh:targetClass uml:TransitionTarget ;
	sh:property [ 
		sh:path uml:TransitionTarget-hasSource ;
		sh:class [ owl:unionOf( uml:Transition FMC:Actor )] ;
		sh:minCount 1 ;
		sh:maxCount 1
	] ;
	sh:property [ 
		sh:path uml:TransitionTarget-hasTarget ;
		sh:class [ owl:unionOf( uml:State FMC:State )] ;
		sh:minCount 1 ;
		sh:maxCount 1
	] .

SpecIF:isSpecializationOf
	rdfs:subClassOf pig:Relationship ;
	rdfs:label "specializes"@en ;
	rdfs:label "spezialisiert"@de ;
	rdfs:label "spécialise"@fr ;
	rdfs:comment "<p>A FMC:Actor is a specialization of another FMC:Actor; similarly for FMC:State and FMC:Event.</p>"@en ;
	dcterms:modified "2024-07-17T15:12:53.003Z" .

SpecIF:isSpecializationOf-hasSource
	rdfs:subPropertyOf pig:eligibleSource ;
	rdfs:label "Connects the source of SpecIF:isSpecializationOf" ;
	rdfs:domain SpecIF:isSpecializationOf ;
	dcterms:modified "2024-07-17T15:12:53.003Z" .

SpecIF:isSpecializationOf-hasTarget
	rdfs:subPropertyOf pig:eligibleTarget ;
	rdfs:label "Connects the target of SpecIF:isSpecializationOf" ;
	rdfs:domain SpecIF:isSpecializationOf ;
	dcterms:modified "2024-07-17T15:12:53.003Z" .

SpecIF:isSpecializationOf-Shape
	sh:targetClass SpecIF:isSpecializationOf ;
	sh:property [ 
		sh:path SpecIF:isSpecializationOf-hasSource ;
		sh:minCount 1 ;
		sh:maxCount 1
	] ;
	sh:property [ 
		sh:path SpecIF:isSpecializationOf-hasTarget ;
		sh:minCount 1 ;
		sh:maxCount 1
	] .

uml:Generalization
	rdfs:subClassOf SpecIF:relates ;
	rdfs:label "generalizes"@en ;
	rdfs:label "generalisiert"@de ;
	rdfs:label "generalise"@fr ;
	rdfs:comment "<p>A [[FMC:Actor]] is a generalization of another [[FMC:Actor]]; similarly for [[FMC:State]] and [[FMC:Event]].</p>"@en ;
	dcterms:modified "2024-06-17T10:03:39.762Z" .

uml:Generalization-hasSource
	rdfs:subPropertyOf pig:eligibleSource ;
	rdfs:label "Connects the source of uml:Generalization" ;
	rdfs:domain uml:Generalization ;
	dcterms:modified "2024-06-17T10:03:39.762Z" .

uml:Generalization-hasTarget
	rdfs:subPropertyOf pig:eligibleTarget ;
	rdfs:label "Connects the target of uml:Generalization" ;
	rdfs:domain uml:Generalization ;
	dcterms:modified "2024-06-17T10:03:39.762Z" .

uml:Generalization-Shape
	sh:targetClass uml:Generalization ;
	sh:property dcterms:type-Shape ;
	sh:property [ 
		sh:path uml:Generalization-hasSource ;
		sh:minCount 1 ;
		sh:maxCount 1
	] ;
	sh:property [ 
		sh:path uml:Generalization-hasTarget ;
		sh:minCount 1 ;
		sh:maxCount 1
	] .

SpecIF:inheritsFrom
	rdfs:subClassOf pig:Relationship ;
	rdfs:label "inherits from"@en ;
	rdfs:label "erbt von"@de ;
	rdfs:label "hérite de"@fr ;
	rdfs:comment "A model-element class inherits from another. For example a data-object of class [[FMC:State]] inherits from another data-object, as shown in a UML Class Diagram). "@en ;
	dcterms:modified "2025-09-05T12:31:56.070Z" .

SpecIF:inheritsFrom-hasSource
	rdfs:subPropertyOf pig:eligibleSource ;
	rdfs:label "Connects the source of SpecIF:inheritsFrom" ;
	rdfs:domain SpecIF:inheritsFrom ;
	dcterms:modified "2025-09-05T12:31:56.070Z" .

SpecIF:inheritsFrom-hasTarget
	rdfs:subPropertyOf pig:eligibleTarget ;
	rdfs:label "Connects the target of SpecIF:inheritsFrom" ;
	rdfs:domain SpecIF:inheritsFrom ;
	dcterms:modified "2025-09-05T12:31:56.070Z" .

SpecIF:inheritsFrom-Shape
	sh:targetClass SpecIF:inheritsFrom ;
	sh:property [ 
		sh:path SpecIF:inheritsFrom-hasSource ;
		sh:minCount 1 ;
		sh:maxCount 1
	] ;
	sh:property [ 
		sh:path SpecIF:inheritsFrom-hasTarget ;
		sh:minCount 1 ;
		sh:maxCount 1
	] .

IR:approves
	rdfs:subClassOf pig:Relationship ;
	rdfs:label "supports"@en ;
	rdfs:label "unterstützt"@de ;
	rdfs:label "soutient"@fr ;
	dcterms:modified "2023-08-09T21:40:04.757Z" .

IR:approves-hasSource
	rdfs:subPropertyOf pig:eligibleSource ;
	rdfs:label "Connects the source of IR:approves" ;
	rdfs:domain IR:approves ;
	dcterms:modified "2023-08-09T21:40:04.757Z" .

IR:approves-hasTarget
	rdfs:subPropertyOf pig:eligibleTarget ;
	rdfs:label "Connects the target of IR:approves" ;
	rdfs:domain IR:approves ;
	rdfs:range SpecIF:Comment ;
	dcterms:modified "2023-08-09T21:40:04.757Z" .

IR:approves-Shape
	sh:targetClass IR:approves ;
	sh:property [ 
		sh:path IR:approves-hasSource ;
		sh:minCount 1 ;
		sh:maxCount 1
	] ;
	sh:property [ 
		sh:path IR:approves-hasTarget ;
		sh:class SpecIF:Comment ;
		sh:minCount 1 ;
		sh:maxCount 1
	] .

IR:opposes
	rdfs:subClassOf pig:Relationship ;
	rdfs:label "opposes"@en ;
	rdfs:label "hemmt"@de ;
	rdfs:label "s'oppose à"@fr ;
	dcterms:modified "2023-08-09T21:40:29.719Z" .

IR:opposes-hasSource
	rdfs:subPropertyOf pig:eligibleSource ;
	rdfs:label "Connects the source of IR:opposes" ;
	rdfs:domain IR:opposes ;
	dcterms:modified "2023-08-09T21:40:29.719Z" .

IR:opposes-hasTarget
	rdfs:subPropertyOf pig:eligibleTarget ;
	rdfs:label "Connects the target of IR:opposes" ;
	rdfs:domain IR:opposes ;
	rdfs:range SpecIF:Comment ;
	dcterms:modified "2023-08-09T21:40:29.719Z" .

IR:opposes-Shape
	sh:targetClass IR:opposes ;
	sh:property [ 
		sh:path IR:opposes-hasSource ;
		sh:minCount 1 ;
		sh:maxCount 1
	] ;
	sh:property [ 
		sh:path IR:opposes-hasTarget ;
		sh:class SpecIF:Comment ;
		sh:minCount 1 ;
		sh:maxCount 1
	] .

DDP:definedBy
	rdfs:subClassOf pig:Relationship ;
	rdfs:label "defined by"@en ;
	rdfs:label "definiert von"@de ;
	rdfs:label "defini par"@fr ;
	dcterms:modified "2025-08-15T14:48:20.668Z" .

DDP:definedBy-hasSource
	rdfs:subPropertyOf pig:eligibleSource ;
	rdfs:label "Connects the source of DDP:definedBy" ;
	rdfs:domain DDP:definedBy ;
	dcterms:modified "2025-08-15T14:48:20.668Z" .

DDP:definedBy-hasTarget
	rdfs:subPropertyOf pig:eligibleTarget ;
	rdfs:label "Connects the target of DDP:definedBy" ;
	rdfs:domain DDP:definedBy ;
	rdfs:range DDP:Source ;
	dcterms:modified "2025-08-15T14:48:20.668Z" .

DDP:definedBy-Shape
	sh:targetClass DDP:definedBy ;
	sh:property [ 
		sh:path DDP:definedBy-hasSource ;
		sh:minCount 1 ;
		sh:maxCount 1
	] ;
	sh:property [ 
		sh:path DDP:definedBy-hasTarget ;
		sh:class DDP:Source ;
		sh:minCount 1 ;
		sh:maxCount 1
	] .

#################################################################
# Entities
#################################################################

d:R-U1OpjV5EE1qmXsAGNWQVCqwH2tC
	rdf:type DDP:ProductFunction ;
	rdfs:label "Customer Relationship Management (CRM)" ;
	rdfs:comment "The app The app provide the ability to create, read, update and delete customers with their- contact person (full name)*- postal address- e-mail address*- telephone number- bank account" ;
	dcterms:modified "2025-09-24T13:54:36.309Z" .

d:R-XCp5i5we6N1zoBSIDhliTgLBPvQ
	rdf:type IREB:Requirement ;
	rdfs:label "App manages customers" ;
	rdfs:comment "The app MUST provide the ability to create, read, update and delete customer information." ;
	SpecIF:Priority SpecIF:priorityRatherHigh ;
	IREB:RequirementType o:V_RequirementType_0 ;
	SpecIF:StakeholderGroup SpecIF:StakeholderGroupBusiness ;
	dcterms:modified "2025-09-24T13:55:25.069Z" .

#################################################################
# Relationships
#################################################################

d:S-w45GuxjUCE5YqFDR2VCjmL7KezD
	rdf:type oslc_rm:satisfies ;
	oslc_rm:satisfies-hasSource d:R-U1OpjV5EE1qmXsAGNWQVCqwH2tC ;
	oslc_rm:satisfies-hasTarget d:R-XCp5i5we6N1zoBSIDhliTgLBPvQ ;
	dcterms:modified "2025-09-24T13:55:42.088Z" .

#################################################################
# Hierarchies
#################################################################

d:HierarchyRoot
	rdf:type pig:HierarchyRoot ;
	rdfs:label "Hierarchy Root" ;
	rdfs:comment "... anchoring all hierarchies of this graph (project)" ;
	pig:lists d:N-3EdYCBmd4SpVXQRxp55oBIro3AO ,
		d:N-IP5BCRHWkyogl3g3cOodDsj93zw .

d:N-3EdYCBmd4SpVXQRxp55oBIro3AO
	dcterms:modified "2025-09-24T13:54:36.309Z" ;
	pig:lists d:R-U1OpjV5EE1qmXsAGNWQVCqwH2tC .

d:N-IP5BCRHWkyogl3g3cOodDsj93zw
	dcterms:modified "2025-09-24T13:55:25.069Z" ;
	pig:lists d:R-XCp5i5we6N1zoBSIDhliTgLBPvQ .
